theories/Lambda/AutoSetoidRewriteRtac.v
@@ -64,7 +64,17 @@ Section setoid.
       t1 = t2.
 
 
-  (** This is the monad that we'll be working with *)
+  (** This monad abstracts the idea of working under a context.
+   ** It is morally exactly the same as [rtac] except for two differences:
+   ** 1) It is generalized over the goal representation so it can avoid
+   **    manifesting [Goal]s
+   ** 2) It has an extra [tvs'] argument that allows it to avoid pushing
+   **    terms into the context when it does not need to.
+   **
+   ** TODO(gmalecha):
+   **   This should be unified with the [rtac] monad but understanding
+   **   the full design still requires a bit more work.
+   **)
   Definition mrw (T : Type) : Type :=
     tenv typ -> tenv typ -> tenv typ -> nat -> nat ->
     forall c : Ctx typ (expr typ func), ctx_subst c ->
@@ -91,6 +101,49 @@ Section setoid.
     fun tvs' tus tvs nus nvs ctx cs =>
       None.
 
+  Definition rw_bind_catch {T U : Type} (c : mrw T) (k : T -> mrw U)
+             (otherwise : mrw U)
+  : mrw U :=
+    fun tus' tus tvs nus nvs ctx cs =>
+      match c tus' tus tvs nus nvs ctx cs with
+      | None => otherwise tus' tus tvs nus nvs ctx cs
+      | Some (val,cs') => k val tus' tus tvs nus nvs ctx cs'
+      end.
+
+  Lemma rw_orelse_case
+  : forall (T : Type) (A B : mrw T) a b c d e f g h,
+      @rw_orelse _ A B a b c d e f g = h ->
+      A a b c d e f g = h \/
+      B a b c d e f g = h.
+  Proof using.
+    unfold rw_orelse. intros.
+    forward.
+  Qed.
+
+  Lemma rw_bind_catch_case
+  : forall (T U : Type) (A : mrw T) (B : T -> mrw U) (C : mrw U)
+           a b c d e f g h,
+      @rw_bind_catch _ _ A B C a b c d e f g = h ->
+      (exists x g', A a b c d e f g = Some (x,g') /\
+                    B x a b c d e f g' = h) \/
+      (C a b c d e f g = h /\ A a b c d e f g = None).
+  Proof using.
+    unfold rw_bind_catch. intros; forward.
+    left. do 2 eexists; split; eauto.
+  Qed.
+
+  Lemma rw_bind_case
+  : forall (T U : Type) (A : mrw T) (B : T -> mrw U)
+           a b c d e f g h,
+      @rw_bind _ _ A B a b c d e f g = Some h ->
+      exists x g',
+        A a b c d e f g = Some (x, g') /\
+        B x a b c d e f g' = Some h.
+  Proof using.
+    unfold rw_bind. intros; forward.
+    do 2 eexists; eauto.
+  Qed.
+
   Section rw_map2.
     Context {T U V : Type}.
     Variable f : T -> U -> mrw V.
@@ -106,16 +159,104 @@ Section setoid.
       end.
   End rw_map2.
 
+  Definition mrw_equiv {T} (rT : T -> T -> Prop) (l : mrw T) (r : mrw T)
+  : Prop :=
+    forall a b c d e f g,
+      Roption (Eqpair rT eq) (l a b c d e f g) (r a b c d e f g).
+
+  Instance Reflexive_mrw_equiv {T} (rT : T -> T -> Prop)
+           {Refl_rT : Reflexive rT}
+  : Reflexive (mrw_equiv rT).
+  Proof using.
+    red. red. intros. eapply Reflexive_Roption. eapply Reflexive_Eqpair; eauto.
+  Qed.
+
+  Instance Symmetric_mrw_equiv {T} (rT : T -> T -> Prop)
+           {Sym_rT : Symmetric rT}
+  : Symmetric (mrw_equiv rT).
+  Proof using.
+    red. red. intros. eapply Symmetric_Roption. eapply Symmetric_Eqpair; eauto.
+    eapply H.
+  Qed.
+
+  Instance Transitive_mrw_equiv {T} (rT : T -> T -> Prop)
+           {Trans_rT : Transitive rT}
+  : Transitive (mrw_equiv rT).
+  Proof using.
+    red. red. intros. eapply Transitive_Roption.
+    eapply Transitive_Eqpair; eauto with typeclass_instances.
+    eapply H. eapply H0.
+  Qed.
+
+  Lemma rw_bind_assoc
+  : forall {T U V} (c : mrw T) (k : T -> mrw U) (k' : U -> mrw V),
+      mrw_equiv eq
+                (rw_bind (rw_bind c k) k')
+                (rw_bind c (fun x => rw_bind (k x) k')).
+  Proof using.
+    unfold rw_bind. simpl.
+    red. intros.
+    destruct (c a b c0 d e f g); try constructor.
+    destruct p.
+    eapply Reflexive_Roption. apply Reflexive_Eqpair; eauto.
+  Qed.
+
+  Lemma rw_bind_rw_ret
+  : forall {T U} (x : T) (k : T -> mrw U),
+      rw_bind (rw_ret x) k = k x.
+  Proof using. reflexivity. Qed.
+
+  Lemma rw_bind_rw_fail
+  : forall {T U} (k : T -> mrw U),
+      rw_bind rw_fail k = rw_fail.
+  Proof using. reflexivity. Qed.
+
+  Lemma Proper_rw_bind (T U : Type)
+  : Proper (mrw_equiv (@eq T) ==> (pointwise_relation (mrw_equiv (@eq U))) ==>
+            mrw_equiv (@eq U)) (@rw_bind T U).
+  Proof using.
+    red. red. red. red. unfold rw_bind. intros.
+    red in H.
+    specialize (H a b c d e f g).
+    destruct H. constructor.
+    destruct H. subst.
+    eapply H0.
+  Qed.
+
+  Instance Injective_mrw_equiv_rw_ret {T} (rT : T -> T -> Prop) (a b : T)
+  : Injective (mrw_equiv rT (rw_ret a) (rw_ret b)) :=
+  { result := rT a b }.
+  Proof using.
+    unfold rw_ret. intros. red in H.
+    specialize (H nil nil nil 0 0 _ (@TopSubst _ _ nil nil)).
+    inv_all. assumption.
+  Defined.
+  (** End of monad definitions **)
+
+  (* [Progressing T] = [option T] but adds the information that the result
+   * makes progress or does not, i.e. a [Progressing T] is relative to an
+   * input [in]. If the output is [NoProgress] then the meaning is the same as
+   * the input, if the result is [Progress x] then [x] is assumed to be
+   * different than [in].
+   *)
   Inductive Progressing (T : Type) : Type :=
   | Progress (new_val : T)
   | NoProgress.
 
   Arguments NoProgress {_}.
 
-  Let rewrite_expr :=
-    forall (es : list (expr typ func * (R -> mrw (Progressing (expr typ func)))))
-           (rg : R),
-      mrw (Progressing (expr typ func)).
+  Definition ProgressD {T} (a : T) (x : Progressing T) : T :=
+    match x with
+    | Progress x => x
+    | NoProgress => a
+    end.
+
+  Definition fmap_Progressing {T U : Type} (f : T -> U) (x : Progressing T)
+    : Progressing U :=
+    match x with
+    | NoProgress => NoProgress
+    | Progress x => Progress (f x)
+    end.
 
   Local Existing Instance Subst_ctx_subst.
   Local Existing Instance SubstOk_ctx_subst.
@@ -124,14 +265,17 @@ Section setoid.
   Local Existing Instance Expr_expr.
   Local Existing Instance ExprOk_expr.
 
-  Definition ProgressD {T} (a : T) (x : Progressing T) : T :=
-    match x with
-    | Progress x => x
-    | NoProgress => a
-    end.
+  (** These are the core specifications. **)
+  (****************************************)
 
+  (* [setoid_rewrite_rel e r rw] states that if [rw] is run on any context that
+   * [e] is well-typed in, then the final context will extend the initial
+   * context and the result will be related at [r]
+   *)
   Definition setoid_rewrite_rel
-             (e : expr typ func) (r : R) (rw : mrw (Progressing (expr typ func))) : Prop :=
+             (e : expr typ func) (r : R)
+             (rw : mrw (Progressing (expr typ func)))
+  : Prop :=
     forall (ctx : Ctx typ (expr typ func)) cs (tvs' : tenv typ) cs'
            (e' : Progressing (expr typ func)),
       let tus := getUVars ctx in
@@ -161,11 +305,22 @@ Section setoid.
       | Some _ , Some _ , Some _ , None => False
       end.
 
+  (* [setoid_rewrite_spec rw] simply states that [rw] is sound for every
+   * [e] and [r].
+   *)
   Definition setoid_rewrite_spec
              (rw : expr typ func -> R -> mrw (Progressing (expr typ func)))
   : Prop :=
     forall e r, @setoid_rewrite_rel e r (rw e r).
 
+  (* This definition is used for recursive rewriting, it computes a list of
+   * sufficient relations to rewrite in the arguments. It is specialized to
+   * justify termination.
+   *   [respectful_spec resp] states that [resp e r = rs] implies
+   *   [Proper (rs ==> r) e]
+   * TODO(gmalecha):
+   *   This can be generalized a bit to support changing the result argument
+   *)
   Definition respectful_spec (respectful : expr typ func -> R -> mrw (list R))
   : Prop :=
     forall tvs' (ctx : Ctx typ (expr typ func)) cs cs' e r rs,
@@ -195,161 +350,60 @@ Section setoid.
       | Some _ , Some _ , Some _ , None => False
       end.
 
+  (** This is the core of the rewriter which applies respectful and performs
+   ** recursive rewriting.
+   **)
   Section setoid_rewrite.
+    Definition arg_rewriter : Type :=
+      expr typ func * (R -> mrw (Progressing (expr typ func))).
+
+    (* This structure is similar in spirit to hereditary substitutions where
+     * arguments are paired with the functions used to rewrite them. This allows
+     * for recursive rewriting without manifesting well-foundedness proofs.
+     *)
     Variable respectfulness
-    : expr typ func -> rewrite_expr.
+    : expr typ func ->
+      forall (es : list arg_rewriter)
+             (rg : R),
+        mrw (Progressing (expr typ func)).
 
-    Definition fmap_Progressing {T U : Type} (f : T -> U) (x : Progressing T)
-    : Progressing U :=
-      match x with
-      | NoProgress => NoProgress
-      | Progress x => Progress (f x)
-      end.
-
-    Fixpoint setoid_rewrite' (e : expr typ func)
-             (es : list (expr typ func * (R -> mrw (Progressing (expr typ func))))) (rg : R)
+    (* This is the core rewriter.
+     *   [setoid_rewrite' e es r] performs rewriting on [e @ es] with respect
+     *   to relation [r].
+     *)
+    Fixpoint setoid_rewrite'
+             (e : expr typ func) (es : list arg_rewriter) (rg : R)
     : mrw (Progressing (expr typ func)) :=
       match e with
-        | App f x =>
-          setoid_rewrite' f ((x, setoid_rewrite' x nil) :: es) rg
-        | Abs t e' =>
-          match es with
-            | nil =>
-              match rg with
-              | Rpointwise _t (*=t*) rg' =>
-                fun tvs tus tvs' nus nvs c cs =>
-                  match @setoid_rewrite' e' nil rg'
-                                         (t::tvs) tus tvs' nus nvs c cs
-                  with
-                  | Some (e'',cs'') =>
-                    Some (fmap_Progressing (Abs t) e'', cs'')
-                  | None => None
-                  end
-              | _ => respectfulness (Abs t e') es rg
+      | App f x =>
+        setoid_rewrite' f ((x, setoid_rewrite' x nil) :: es) rg
+      | Abs t e' =>
+        match es with
+        | nil =>
+          match rg with
+          | Rpointwise _t (*=t*) rg' =>
+            fun tvs tus tvs' nus nvs c cs =>
+              match @setoid_rewrite' e' nil rg'
+                                     (t::tvs) tus tvs' nus nvs c cs
+              with
+              | Some (e'',cs'') =>
+                Some (fmap_Progressing (Abs t) e'', cs'')
+              | None => None
               end
-            | _ => respectfulness (Abs t e') es rg
+          | _ => respectfulness (Abs t e') es rg
           end
-        | Var v => respectfulness (Var v) es rg
-        | UVar u => respectfulness (UVar u) es rg
-        | Inj i => respectfulness (Inj i) es rg
+        | _ => respectfulness (Abs t e') es rg
+        end
+      | Var v => respectfulness (Var v) es rg
+      | UVar u => respectfulness (UVar u) es rg
+      | Inj i => respectfulness (Inj i) es rg
       end.
 
     Definition setoid_rewrite (e : expr typ func) (rg : R)
     : mrw (Progressing (expr typ func)) :=
       setoid_rewrite' e nil rg.
 
-    Let _lookupU (u : ExprI.uvar) : option (expr typ func) := None.
-    Let _lookupV (under : nat) (above : nat) (v : ExprI.var)
-    : option (expr typ func) :=
-      Some (Var (if v ?[ ge ] under then
-                   v - under
-                 else
-                   v + above)).
-
-    Definition expr_convert (u : nat) (above : nat)
-    : expr typ func -> expr typ func :=
-      expr_subst _lookupU (_lookupV u above) 0.
-
-    (** TODO(gmalecha): Move to EnvI or ExtLib.Data.HList **)
-    Lemma nth_error_get_hlist_nth_appR'
-    : forall T (F : T -> Type) ls u v,
-        nth_error_get_hlist_nth F ls u = Some v ->
-        forall ls',
-        exists v',
-          nth_error_get_hlist_nth F (ls' ++ ls) (u + length ls') = Some (existT _ (projT1 v) v') /\
-          forall a b,
-            projT2 v a = v' (hlist_app b a).
-    Proof using.
-      induction ls'.
-      { simpl.
-        replace (u + 0) with u by omega.
-        destruct v. eexists; split; eauto.
-        simpl. intros.
-        rewrite (hlist_eta b). reflexivity. }
-      { simpl.
-        replace (u + S (length ls')) with (S (u + length ls')) by omega.
-        destruct IHls' as [ ? [ ? ? ] ].
-        rewrite H0. eexists; split; eauto.
-        simpl. intros.
-        rewrite (hlist_eta b). simpl. eauto. }
-    Qed.
-
-    Lemma expr_convert_sound
-    : forall tus tvs tvs' e t eD,
-        exprD' tus (tvs ++ tvs') t e = Some eD ->
-        exists eD',
-          exprD' tus (tvs' ++ tvs) t (expr_convert (length tvs) (length tvs') e) = Some eD' /\
-          forall a b c,
-            eD a (hlist_app b c) = eD' a (hlist_app c b).
-    Proof.
-      clear - Typ2Ok_Fun RTypeOk_typD RSymOk_func.
-      unfold expr_convert.
-      intros.
-      destruct (fun Hu Hv => @ExprI.expr_subst_sound
-                    typ _ (expr typ func) (Expr_expr _ _ _ _) _
-                    _lookupU
-                    (_lookupV (length tvs) (length tvs'))
-                    0 e _ eq_refl nil
-                    tus (tvs ++ tvs') tus (tvs' ++ tvs)
-                    (fun us vs us' vs' =>
-                       us = us' /\
-                       let (_vs,_vs') := hlist_split _ _ vs in
-                       let (__vs,__vs') := hlist_split _ _ vs' in
-                       _vs = __vs' /\ _vs' = __vs) Hu Hv t _ eq_refl H).
-      { simpl. clear.
-        intros. eexists; split; eauto.
-        intros. destruct H1; subst; auto. }
-      { simpl. intros.
-        autorewrite with exprD_rw. simpl.
-        consider (u ?[ ge ] length tvs); intros.
-        { eapply nth_error_get_hlist_nth_appR in H1; eauto.
-          simpl in H1. forward_reason.
-          eapply nth_error_get_hlist_nth_weaken with (ls':=tvs) in H1.
-          simpl in H1.
-          forward_reason. rewrite H1.
-          rewrite type_cast_refl; eauto.
-          eexists; split; eauto.
-          unfold Rcast_val, Rcast, Relim. simpl.
-          intros.
-          revert H5.
-          rewrite <- (hlist_app_hlist_split _ _ vs).
-          rewrite <- (hlist_app_hlist_split _ _ vs').
-          rewrite hlist_split_hlist_app.
-          rewrite hlist_split_hlist_app.
-          destruct 1.
-          rewrite H3. rewrite <- H4.
-          f_equal. tauto. }
-        { assert (u < length tvs) by omega.
-          eapply nth_error_get_hlist_nth_appL in H3.
-          destruct H3. destruct H3.
-          rewrite H3 in H1.
-          assert (u + length tvs' >= length tvs') by omega.
-          destruct H4 as [ ? [ ? ? ] ].
-          eapply nth_error_get_hlist_nth_appR' in H4; simpl in H4.
-          destruct H4 as [ ? [ ? ? ] ].
-          rewrite H4.
-          inv_all. subst. simpl.
-          rewrite type_cast_refl; eauto.
-          eexists; split; eauto.
-          intros us vs us' vs'.
-          rewrite <- (hlist_app_hlist_split _ _ vs).
-          rewrite <- (hlist_app_hlist_split _ _ vs').
-          rewrite hlist_split_hlist_app.
-          rewrite hlist_split_hlist_app.
-          destruct 1.
-          simpl in *.
-          rewrite H6. rewrite <- H7.
-          unfold Rcast_val, Rcast; simpl. f_equal. tauto. } }
-      { simpl in H0.
-        destruct H0; eexists; split; eauto.
-        intros. apply (H1 a (hlist_app b c) a (hlist_app c b) Hnil).
-        split; auto.
-        do 2 rewrite hlist_split_hlist_app.
-        tauto. }
-    Qed.
-
-    Definition setoid_rewrite_rec
-      (ls : list (expr typ func * (R -> mrw (Progressing (expr typ func)))))
+    Definition setoid_rewrite_rec (ls : list arg_rewriter)
     : Prop :=
       Forall (fun e =>
                 forall r,
@@ -477,74 +531,8 @@ Section setoid.
       rewrite H. rewrite H0. reflexivity.
     Qed.
 
-    (** TODO: Move **)
-    Fixpoint apply_fold tus tvs t ts
-             (es : HList.hlist (fun t => ExprI.exprT tus tvs (typD t)) ts)
-    : ExprI.exprT tus tvs (typD (fold_right (typ2 (F:=RFun)) t ts))
-      -> ExprI.exprT tus tvs (typD t) :=
-      match es in HList.hlist _ ts
-            return ExprI.exprT tus tvs (typD (fold_right (typ2 (F:=RFun)) t ts))
-                   -> ExprI.exprT tus tvs (typD t)
-      with
-      | HList.Hnil => fun f => f
-      | HList.Hcons x xs => fun f =>
-                              @apply_fold tus tvs t _ xs (AbsAppI.exprT_App f x)
-      end.
-
-    (** TODO: Move **)
-    Lemma apps_exprD'_fold_type
-    : forall tus tvs es e t eD,
-        exprD' tus tvs t (apps e es) = Some eD ->
-        exists ts fD esD,
-          exprD' tus tvs (fold_right (typ2 (F:=RFun)) t ts) e = Some fD /\
-          hlist_build (fun t => ExprI.exprT tus tvs (typD t))
-                      (fun t e => exprD' tus tvs t e) ts es = Some esD /\
-          forall us vs,
-            eD us vs = @apply_fold _ _ _ _ esD fD us vs.
-    Proof.
-      clear - Typ2Ok_Fun RTypeOk_typD RSymOk_func.
-      intros.
-      rewrite exprD'_apps in H; eauto.
-      unfold apps_sem' in H. forward. clear H.
-      revert H0; revert H1; revert eD; revert t; revert e0; revert e.
-      revert t0.
-      induction es; simpl; intros.
-      { exists nil. exists eD. exists HList.Hnil.
-        simpl. split; eauto.
-        forward. destruct r. inv_all; subst. assumption. }
-      { arrow_case_any.
-        { clear H.
-          red in x1. subst.
-          simpl in H1. autorewrite_with_eq_rw_in H1.
-          forward; inv_all; subst.
-          eapply IHes with (e := App e a) in H3; eauto.
-          { forward_reason.
-            assert (x0 = fold_right (typ2 (F:=RFun)) t x1).
-            { autorewrite with exprD_rw in H2; simpl in H2.
-              rewrite (exprD_typeof_Some _ _ _ _ _ H) in H2.
-              rewrite H in H2.
-              forward; inv_all; subst.
-              eapply exprD_typeof_Some in H2; eauto.
-              eapply exprD_typeof_Some in H0; eauto.
-              rewrite H0 in H2.
-              inv_all. assumption. }
-            { subst.
-              eexists (x :: x1). exists e0.
-              eexists. split; eauto.
-              split.
-              { simpl.
-                rewrite H3. rewrite H. reflexivity. }
-              { simpl. intros.
-                erewrite exprD'_App in H2; eauto.
-                inv_all; subst. eauto. } } }
-          { erewrite exprD'_App; eauto.
-            unfold AbsAppI.exprT_App. autorewrite_with_eq_rw.
-            reflexivity. } }
-        { inversion H1. } }
-    Qed.
-
     Fixpoint recursive_rewrite' (prog : bool) (f : expr typ func)
-             (es : list (expr typ func * (R -> mrw (Progressing (expr typ func)))))
+             (es : list arg_rewriter)
              (rs : list R)
     : mrw (Progressing (expr typ func)) :=
       match es , rs with
@@ -562,1268 +550,6 @@ Section setoid.
       end.
 
     Definition recursive_rewrite := recursive_rewrite' false.
-
-    Definition mrw_equiv {T} (rT : T -> T -> Prop) (l : mrw T) (r : mrw T)
-    : Prop :=
-      forall a b c d e f g,
-        Roption (Eqpair rT eq) (l a b c d e f g) (r a b c d e f g).
-
-    Instance Reflexive_mrw_equiv {T} (rT : T -> T -> Prop)
-             {Refl_rT : Reflexive rT}
-    : Reflexive (mrw_equiv rT).
-    Proof using.
-      red. red. intros. eapply Reflexive_Roption. eapply Reflexive_Eqpair; eauto.
-    Qed.
-
-    Instance Symmetric_mrw_equiv {T} (rT : T -> T -> Prop)
-             {Sym_rT : Symmetric rT}
-    : Symmetric (mrw_equiv rT).
-    Proof using.
-      red. red. intros. eapply Symmetric_Roption. eapply Symmetric_Eqpair; eauto.
-      eapply H.
-    Qed.
-
-    Instance Transitive_mrw_equiv {T} (rT : T -> T -> Prop)
-             {Trans_rT : Transitive rT}
-    : Transitive (mrw_equiv rT).
-    Proof using.
-      red. red. intros. eapply Transitive_Roption.
-      eapply Transitive_Eqpair; eauto with typeclass_instances.
-      eapply H. eapply H0.
-    Qed.
-
-    Lemma rw_bind_assoc
-    : forall {T U V} (c : mrw T) (k : T -> mrw U) (k' : U -> mrw V),
-        mrw_equiv eq
-                  (rw_bind (rw_bind c k) k')
-                  (rw_bind c (fun x => rw_bind (k x) k')).
-    Proof using.
-      unfold rw_bind. simpl.
-      red. intros.
-      destruct (c a b c0 d e f g); try constructor.
-      destruct p.
-      eapply Reflexive_Roption. apply Reflexive_Eqpair; eauto.
-    Qed.
-
-    Lemma Proper_rw_bind (T U : Type)
-    : Proper (mrw_equiv (@eq T) ==> (pointwise_relation (mrw_equiv (@eq U))) ==> mrw_equiv (@eq U)) (@rw_bind T U).
-    Proof using.
-      red. red. red. red. unfold rw_bind. intros.
-      red in H.
-      specialize (H a b c d e f g).
-      destruct H. constructor.
-      destruct H. subst.
-      eapply H0.
-    Qed.
-
-    Lemma rw_bind_rw_ret
-    : forall {T U} (x : T) (k : T -> mrw U),
-        rw_bind (rw_ret x) k = k x.
-    Proof using. reflexivity. Qed.
-
-    Lemma rw_bind_rw_fail
-    : forall {T U} (k : T -> mrw U),
-        rw_bind rw_fail k = rw_fail.
-    Proof using. reflexivity. Qed.
-
-    (** Note, this is quite inefficient due to building and destructing
-     ** the pair
-     **)
-    Fixpoint extend_ctx (tvs' : tenv typ)
-             (ctx : Ctx typ (expr typ func)) (cs : ctx_subst ctx) {struct tvs'}
-    : { ctx : Ctx typ (expr typ func) & ctx_subst ctx } :=
-      match tvs' with
-      | nil => @existT _ _ ctx cs
-      | t :: tvs' =>
-        match @extend_ctx tvs' ctx cs with
-        | existT _ ctx' cs' => @existT _ _ (CAll ctx' t) (AllSubst cs')
-        end
-      end.
-
-    Definition core_rewrite (lem : rw_lemma typ func Rbase)
-               (tac : rtacK typ (expr typ func))
-    : expr typ func -> tenv typ -> tenv typ -> nat -> nat ->
-      forall c : Ctx typ (expr typ func),
-        ctx_subst c -> option (expr typ func * ctx_subst c) :=
-        match typeof_expr nil lem.(vars) lem.(concl).(lhs) with
-        | None => fun _ _ _ _ _ _ _ => None
-        | Some t =>
-          fun e tus tvs nus nvs ctx cs =>
-           let ctx' := CExs ctx lem.(vars) in
-           let cs' : ctx_subst ctx' := ExsSubst cs (amap_empty _) in
-           let tus' := tus ++ lem.(vars) in
-           match
-             exprUnify 10 tus' tvs 0 (vars_to_uvars 0 nus lem.(concl).(lhs))
-                       e t cs'
-           with
-           | None => None
-           | Some cs'' =>
-             let prems :=
-                 List.map (fun e => GGoal (vars_to_uvars 0 nus e)) lem.(premises)
-             in
-             match
-               tac tus' tvs (length lem.(vars) + nus) nvs ctx' cs'' (GConj_list prems)
-             with
-             | Solved cs''' =>
-               match cs''' in ctx_subst ctx
-                     return match ctx with
-                            | CExs z _ => option (expr typ func * ctx_subst z)
-                            | _ => unit
-                            end
-               with
-               | ExsSubst cs'''' sub =>
-                 if amap_is_full (length lem.(vars)) sub then
-                   let res :=
-                       instantiate (fun u => amap_lookup u sub) 0
-                                   (vars_to_uvars 0 nus lem.(concl).(rhs))
-                   in
-                   Some (res, cs'''')
-                 else
-                   None
-               | _ => tt
-               end
-             | _ => None
-             end
-           end
-        end.
-
-    Definition dtree T : Type := R -> list T.
-
-    Fixpoint rewrite_dtree (ls : list (rw_lemma typ func Rbase * rtacK typ (expr typ func)))
-    : dtree (rw_lemma typ func Rbase * rtacK typ (expr typ func)) :=
-        match ls with
-        | nil => fun _ => nil
-        | (lem,tac) :: ls =>
-          let build := rewrite_dtree ls in
-          fun r =>
-            if Req_dec Rbase_eq r lem.(concl).(rel) then
-              (lem,tac) :: build r
-            else
-              build r
-        end.
-
-    Fixpoint using_rewrite_db' (ls : list (rw_lemma typ func Rbase * rtacK typ (expr typ func)))
-    : expr typ func -> R ->
-      tenv typ -> tenv typ -> nat -> nat ->
-      forall ctx, ctx_subst ctx -> option (expr typ func * ctx_subst ctx) :=
-      match ls with
-      | nil => fun _ _ _ _ _ _ _ _ => None
-      | (lem,tac) :: ls =>
-        let res := using_rewrite_db' ls in
-        let crw := core_rewrite lem tac in
-        fun e r tus tvs nus nvs ctx cs =>
-          if Req_dec Rbase_eq r lem.(concl).(rel) then
-            match crw e tus tvs nus nvs ctx cs with
-            | None => res e r tus tvs nus nvs ctx cs
-            | X => X
-            end
-          else res e r tus tvs nus nvs ctx cs
-      end.
-
-    Fixpoint wrap_tvs (tvs : tenv typ) (ctx : Ctx typ (expr typ func))
-    : Ctx typ (expr typ func) :=
-      match tvs with
-      | nil => ctx
-      | t :: tvs' => wrap_tvs tvs' (CAll ctx t)
-      end.
-
-    Fixpoint wrap_tvs_ctx_subst tvs ctx (cs : ctx_subst ctx)
-    : ctx_subst (wrap_tvs tvs ctx) :=
-      match tvs as tvs return ctx_subst (wrap_tvs tvs ctx) with
-      | nil => cs
-      | t :: tvs => wrap_tvs_ctx_subst _ (AllSubst cs)
-      end.
-
-    Fixpoint unwrap_tvs_ctx_subst T tvs ctx
-    : ctx_subst (wrap_tvs tvs ctx) -> (ctx_subst ctx -> T) -> T :=
-      match tvs as tvs
-            return ctx_subst (wrap_tvs tvs ctx) -> (ctx_subst ctx -> T) -> T
-      with
-      | nil => fun cs k => k cs
-      | t :: tvs => fun cs k =>
-        @unwrap_tvs_ctx_subst T tvs (CAll ctx t) cs (fun z => k (fromAll z))
-      end.
-
-    Lemma getUVars_wrap_tvs
-    : forall tvs' ctx, getUVars (wrap_tvs tvs' ctx) = getUVars ctx.
-    Proof. clear. induction tvs'; simpl; auto.
-           intros.  rewrite IHtvs'. reflexivity.
-    Defined.
-
-    Lemma WellFormed_ctx_subst_wrap_tvs : forall tvs' ctx (cs : ctx_subst ctx),
-        WellFormed_ctx_subst cs ->
-        WellFormed_ctx_subst (wrap_tvs_ctx_subst tvs' cs).
-    Proof using.
-      induction tvs'; simpl; auto.
-      intros. eapply IHtvs'. constructor. assumption.
-    Qed.
-
-    Lemma getAmbientUVars_wrap_tvs : forall tvs ctx,
-        getAmbientUVars (wrap_tvs tvs ctx) = getAmbientUVars ctx.
-    Proof using.
-      induction tvs; simpl. reflexivity.
-      intros. rewrite IHtvs. reflexivity.
-    Defined.
-
-    Lemma getAmbientVars_wrap_tvs : forall tvs ctx,
-        getAmbientVars (wrap_tvs tvs ctx) = getAmbientVars ctx.
-    Proof using.
-      induction tvs; simpl. reflexivity.
-      intros. rewrite IHtvs. reflexivity.
-    Defined.
-
-    Lemma getVars_wrap_tvs : forall tvs' ctx,
-        getVars (wrap_tvs tvs' ctx) = getVars ctx ++ tvs'.
-    Proof using.
-      induction tvs'; simpl; eauto.
-      symmetry. eapply app_nil_r_trans.
-      simpl. intros. rewrite IHtvs'. simpl.
-      rewrite app_ass_trans. reflexivity.
-    Defined.
-
-    Lemma WellFormed_ctx_subst_unwrap_tvs
-    : forall tvs' ctx ctx' (cs : ctx_subst _)
-             (k : ctx_subst (Ctx_append ctx ctx') -> ctx_subst ctx),
-        (forall cs, WellFormed_ctx_subst cs -> WellFormed_ctx_subst (k cs)) ->
-        WellFormed_ctx_subst cs ->
-        WellFormed_ctx_subst
-          (@unwrap_tvs_ctx_subst (ctx_subst ctx) tvs' (Ctx_append ctx ctx') cs k).
-    Proof using.
-      induction tvs'; simpl; auto.
-      intros. specialize (IHtvs' ctx (CAll ctx' a) cs).
-      simpl in *. eapply IHtvs'; eauto.
-      intros. eapply H. rewrite (ctx_subst_eta cs0) in H1.
-      inv_all. assumption.
-    Qed.
-
-    Fixpoint unwrap_tvs_ctx_subst' (tvs : tenv typ) (ctx : Ctx typ (expr typ func))
-    : ctx_subst (wrap_tvs tvs ctx) -> ctx_subst ctx :=
-      match tvs as tvs return ctx_subst (wrap_tvs tvs ctx) -> ctx_subst ctx with
-      | nil => fun X => X
-      | t :: tvs => fun X => fromAll (unwrap_tvs_ctx_subst' tvs _ X)
-      end.
-
-    Theorem unwrap_tvs_ctx_subst_unwrap_tvs_ctx_subst'
-    : forall T tvs ctx cs (k : _ -> T),
-        k (@unwrap_tvs_ctx_subst' tvs ctx cs) =
-        unwrap_tvs_ctx_subst tvs cs k.
-    Proof using.
-      induction tvs; simpl. auto.
-      intros. rewrite <- IHtvs. reflexivity.
-    Qed.
-
-    (** TODO: Move **)
-    Lemma pctxD_iff : forall ctx (cs : ctx_subst ctx) cD P Q,
-        pctxD cs = Some cD ->
-        (forall us vs, P us vs <-> Q us vs) ->
-        forall us vs,
-          cD P us vs <-> cD Q us vs.
-    Proof using.
-      intros.
-      split; eapply Ap_pctxD; eauto; eapply Pure_pctxD; eauto; intros; eapply H0; eauto.
-    Qed.
-
-    (** TODO: Move **)
-    Lemma forall_hlist_nil : forall T (F : T -> Type) (P : hlist F nil -> Prop),
-        (forall x, P x) <-> P Hnil.
-    Proof using.
-      intros. split. eauto. intros. rewrite hlist_eta. assumption.
-    Qed.
-
-    Lemma forall_hlist_cons : forall T (F : T -> Type) t ts (P : hlist F (t :: ts) -> Prop),
-        (forall x, P x) <-> (forall x xs, P (Hcons x xs)).
-    Proof.
-      intros. split. eauto. intros. rewrite hlist_eta. eapply H.
-    Qed.
-
-    Lemma pctxD_unwrap_tvs_ctx_subst
-    : forall tvs ctx (cs : ctx_subst _) cD,
-        pctxD cs = Some cD ->
-        exists cD',
-          pctxD (@unwrap_tvs_ctx_subst _ tvs ctx cs (fun x => x)) = Some cD' /\
-          forall (us : hlist typD _) (vs : hlist typD _) (P : exprT _ _ Prop),
-            cD' (fun us vs => forall vs', P us (hlist_app vs vs')) us vs <->
-            cD match eq_sym (getVars_wrap_tvs tvs ctx) in _ = V
-                   , eq_sym (getUVars_wrap_tvs tvs ctx) in _ = U
-                     return exprT U V Prop
-               with
-               | eq_refl , eq_refl => P
-               end
-               match eq_sym (getAmbientUVars_wrap_tvs tvs ctx) in _ = V
-                     return hlist _ V
-               with
-               | eq_refl => us
-               end
-               match eq_sym (getAmbientVars_wrap_tvs tvs ctx) in _ = V
-                     return hlist _ V
-               with
-               | eq_refl => vs
-               end.
-    Proof.
-      clear - RTypeOk_typD RSymOk_func Typ2Ok_Fun.
-      intros. rewrite <- unwrap_tvs_ctx_subst_unwrap_tvs_ctx_subst'.
-      generalize dependent cD. revert cs. revert ctx.
-      induction tvs.
-      { simpl. eauto.
-        eexists; split; eauto.
-        intros.
-        eapply pctxD_iff; eauto.
-        intros.
-        rewrite forall_hlist_nil.
-        rewrite hlist_app_nil_r.
-        generalize (app_nil_r_trans (getVars ctx)).
-        clear. generalize dependent (getVars ctx ++ nil).
-        intros; subst. reflexivity. }
-      { simpl; intros.
-        specialize (@IHtvs _ _ _ H).
-        forward_reason.
-        generalize dependent (unwrap_tvs_ctx_subst' tvs (CAll ctx a) cs).
-        intro. rewrite (ctx_subst_eta c); simpl.
-        intros; forwardy.
-        eexists; split; eauto.
-        inv_all. subst. intros.
-        specialize (H1 us vs
-                       match eq_sym (app_ass_trans (getVars ctx) (a::nil) _) in _ = X
-                             return exprT _ X Prop
-                       with
-                       | eq_refl => P
-                       end).
-        simpl in *.
-        etransitivity; [ etransitivity; [ | eapply H1 ] | ]; clear H1.
-        { eapply pctxD_iff; eauto.
-          intros.
-          rewrite forall_hlist_cons.
-          eapply Data.Prop.forall_iff; intros.
-          eapply Data.Prop.forall_iff; intros.
-          rewrite hlist_app_assoc.
-          clear. simpl.
-          generalize dependent (app_ass_trans (getVars ctx) (a :: nil) tvs).
-          simpl in *.
-          generalize dependent ((getVars ctx ++ a :: nil) ++ tvs).
-          intros; subst. reflexivity. }
-        { clear - H.
-          match goal with
-          | |- _ _ ?U ?V <-> _ _ ?U' ?V' =>
-            replace V with V' ; [ replace U with U' | ]
-          end.
-          { eapply pctxD_iff; eauto; clear.
-            generalize (app_ass_trans (getVars ctx) (a :: nil) tvs).
-            generalize (getVars_wrap_tvs tvs (CAll ctx a)).
-            generalize (getUVars_wrap_tvs tvs (CAll ctx a)).
-            simpl.
-            intros;
-            repeat match goal with
-               | H : @eq (tenv typ) ?X ?Y |- _ =>
-                 first [ generalize dependent X | generalize dependent Y ] ; intros; subst
-               | H : @eq (list typ) ?X ?Y |- _ =>
-                 first [ generalize dependent X | generalize dependent Y ] ; intros; subst
-               end. reflexivity. }
-          { clear.
-            generalize (getAmbientUVars_wrap_tvs tvs (CAll ctx a)).
-            simpl in *. destruct e. reflexivity. }
-          { clear.
-            generalize (getAmbientVars_wrap_tvs tvs (CAll ctx a)).
-            simpl. destruct e. reflexivity. } } }
-    Qed.
-
-    Lemma pctxD_wrap_tvs_ctx_subst
-    : forall tvs ctx (cs : ctx_subst ctx) cD,
-        pctxD cs = Some cD ->
-        exists cD',
-          pctxD (wrap_tvs_ctx_subst tvs cs) = Some cD' /\
-          forall us vs (P : exprT _ _ Prop),
-            cD (fun us vs => forall vs', P us (hlist_app vs vs')) us vs <->
-            cD' match eq_sym (getVars_wrap_tvs tvs ctx) in _ = V
-                                                           , eq_sym (getUVars_wrap_tvs tvs ctx) in _ = U
-                      return exprT U V Prop
-                with
-                | eq_refl , eq_refl => P
-                end
-                match eq_sym (getAmbientUVars_wrap_tvs tvs ctx) in _ = V
-                      return hlist _ V
-                with
-                | eq_refl => us
-                end
-                match eq_sym (getAmbientVars_wrap_tvs tvs ctx) in _ = V
-                      return hlist _ V
-                with
-                | eq_refl => vs
-                end.
-    Proof using RTypeOk_typD RSymOk_func Typ2Ok_Fun.
-      induction tvs.
-      { simpl. eauto.
-        eexists; split; eauto.
-        intros; eapply pctxD_iff; eauto.
-        intros. rewrite forall_hlist_nil.
-        rewrite hlist_app_nil_r. clear.
-        generalize (app_nil_r_trans (getVars ctx)).
-        generalize dependent (getVars ctx ++ nil). intros; subst.
-        reflexivity. }
-      { simpl. intros.
-        specialize (IHtvs (CAll ctx a) (AllSubst cs)).
-        simpl in IHtvs. rewrite H in IHtvs.
-        specialize (IHtvs _ eq_refl).
-        destruct IHtvs as [ ? [ ? ? ] ].
-        eexists; split; eauto.
-        intros.
-        specialize (H1 us vs
-                       match eq_sym (app_ass_trans (getVars ctx) (a::nil) _) in _ = X
-                             return exprT _ X Prop
-                       with
-                       | eq_refl => P
-                       end).
-        etransitivity; [ etransitivity; [ | eapply H1 ] | ]; clear H1.
-        { eapply pctxD_iff; eauto.
-          intros. rewrite forall_hlist_cons.
-          eapply Data.Prop.forall_iff; intro.
-          eapply Data.Prop.forall_iff; intro.
-          rewrite hlist_app_assoc.
-          clear.
-          generalize dependent (eq_sym (app_ass_trans (getVars ctx) (a :: nil) tvs)).
-          simpl in *. destruct e. reflexivity. }
-        { match goal with
-          | |- _ _ ?U ?V <-> _ _ ?U' ?V' =>
-            replace V with V' ; [ replace U with U' | ]
-          end.
-          { eapply pctxD_iff; eauto.
-            intros.
-            generalize (app_ass_trans (getVars ctx) (a :: nil) tvs).
-            generalize (getVars_wrap_tvs tvs (CAll ctx a)).
-            generalize (getUVars_wrap_tvs tvs (CAll ctx a)).
-            simpl. clear.
-            intros;
-            repeat match goal with
-               | H : @eq (tenv typ) ?X ?Y |- _ =>
-                 first [ generalize dependent X | generalize dependent Y ] ; intros; subst
-               | H : @eq (list typ) ?X ?Y |- _ =>
-                 first [ generalize dependent X | generalize dependent Y ] ; intros; subst
-               end. reflexivity. }
-          { clear.
-            generalize (getAmbientUVars_wrap_tvs tvs (CAll ctx a)).
-            simpl in *. destruct e. reflexivity. }
-          { clear.
-            generalize (getAmbientVars_wrap_tvs tvs (CAll ctx a)).
-            simpl. destruct e. reflexivity. } } }
-    Qed.
-
-    Fixpoint process (r : R) : R * list R :=
-      match r with
-      | Rrespects a b =>
-        let '(x,y) := process b in
-        (x,a::y)
-      | _ => (r, nil)
-      end.
-
-    Fixpoint build_dtree {T} (ls : list (R * T)) : dtree T :=
-      match ls with
-      | nil => fun _ => nil
-      | (r,val) :: ls =>
-        let rest := build_dtree ls in
-        fun r' =>
-          if Req_dec Rbase_eq r r' then val :: rest r' else rest r'
-      end.
-
-    Fixpoint do_respectful
-             (propers : list (expr typ func * R))
-    : expr typ func -> R -> mrw (list R) :=
-      let data := build_dtree (List.map (fun er =>
-                                           let (r,rs) := process (snd er) in
-                                           (r, (fst er, rs))) propers) in
-      let func_cmp x y :=
-          match sym_eqb x y with
-          | Some true => true
-          | _ => false
-          end
-      in
-      fun e r _ _ _ _ _ _ x =>
-        first_success (fun er =>
-                         if expr_eq_sdec (typ:=typ) _ func_cmp e (fst er)
-                         then Some (snd er, x)
-                         else None) (data r).
-
-    Definition do_respectful_poly
-             (polys : expr typ func -> R -> list R)
-    : expr typ func -> R -> mrw (list R) :=
-      fun e r _ _ _ _ _ _ x =>
-        Some (polys e r, x).
-
-    Definition for_tactic
-               (m : expr typ func ->
-                    tenv typ -> tenv typ -> nat -> nat ->
-                    forall ctx : Ctx typ (expr typ func),
-                      ctx_subst ctx -> option (expr typ func * ctx_subst ctx))
-    : expr typ func -> mrw (expr typ func) :=
-      fun e tvs' tus tvs nus nvs ctx cs =>
-        let under := length tvs' in
-        let e' := expr_convert under nvs e in
-        match
-          m e' tus (tvs ++ tvs') nus (under + nvs) _
-            (@wrap_tvs_ctx_subst tvs' ctx cs)
-        with
-        | None => None
-        | Some (v,cs') =>
-          Some (expr_convert nvs under v,
-                @unwrap_tvs_ctx_subst _ tvs' ctx cs' (fun x=> x))
-        end.
-
-    (** Even if we do not need to run a tactic, we still need the
-     ** environment around so that unification will work correctly
-     **)
-    Definition using_rewrite_db
-               (ls : list (rw_lemma typ func Rbase * rtacK typ (expr typ func)))
-    : expr typ func -> R -> mrw (expr typ func) :=
-      let rw_db := using_rewrite_db' ls in
-      fun e r => for_tactic (fun e => rw_db e r) e.
-
-    Definition using_prewrite_db
-        (lems : expr typ func -> list (rw_lemma typ func Rbase * rtacK typ (expr typ func)))
-    : expr typ func -> R -> mrw (expr typ func) :=
-      fun e r =>
-        for_tactic (fun e => using_rewrite_db' (lems e) e r) e.
-
-    (** TODO: Move **)
-    Lemma exprD'_weakenV
-    : forall (tus tvs : tenv typ) (e : expr typ func) (t : typ)
-             (val : exprT tus tvs (typD t)) (tvs' : list typ),
-        exprD' tus tvs t e = Some val ->
-        exists val' : exprT tus (tvs ++ tvs') (typD t),
-          exprD' tus (tvs ++ tvs') t e = Some val' /\
-          (forall (us : hlist typD tus) (vs : hlist typD tvs)
-                  (vs' : hlist typD tvs'),
-              val us vs = val' us (hlist_app vs vs')).
-    Proof.
-      intros.
-      generalize (@exprD'_weakenV typ _ (expr typ func) _ _ tus tvs tvs' e t val H).
-      eauto.
-    Qed.
-
-    (** TODO: Move **)
-    Lemma exprD'_weakenU
-    : forall (tus tvs : tenv typ) (e : expr typ func) (t : typ)
-             (val : exprT tus tvs (typD t)) (tus' : list typ),
-        exprD' tus tvs t e = Some val ->
-        exists val' : exprT (tus ++ tus') tvs (typD t),
-          exprD' (tus ++ tus') tvs t e = Some val' /\
-          (forall (us : hlist typD tus) (vs : hlist typD tvs)
-                  (us' : hlist typD tus'),
-              val us vs = val' (hlist_app us us') vs).
-    Proof.
-      intros.
-      generalize (@exprD'_weakenU typ _ (expr typ func) _ _ tus tus' tvs e t val H).
-      eauto.
-    Qed.
-
-    Existing Instance Reflexive_Roption.
-    Existing Instance Reflexive_RexprT.
-
-    Opaque instantiate.
-
-    (** TODO(gmalecha): Move **)
-    Local Instance Subst_amap T : Subst (amap T) T :=
-      FMapSubst.SUBST.Subst_subst T.
-    Local Instance SubstOk_amap : SubstOk (Subst_amap (expr typ func)) :=
-      @FMapSubst.SUBST.SubstOk_subst typ _ (expr typ func) _.
-
-    (** TODO: Move **)
-    Lemma core_rewrite_sound
-    : forall ctx (cs : ctx_subst ctx),
-        let tus := getUVars ctx in
-        let tvs := getVars ctx in
-        forall l0 r0 e e' cs',
-          rtacK_sound r0 ->
-          lemmaD (rw_conclD RbaseD) nil nil l0 ->
-          core_rewrite l0 r0 e tus tvs (length tus) (length tvs) cs = Some (e', cs') ->
-          WellFormed_ctx_subst cs ->
-          WellFormed_ctx_subst cs' /\
-          (forall (t : typ) (rD : typD t -> typD t -> Prop),
-              RD RbaseD (rel (concl l0)) t = Some rD ->
-              match pctxD cs with
-              | Some _ =>
-                match exprD' tus tvs t e with
-                | Some eD =>
-                  match pctxD cs' with
-                  | Some csD' =>
-                    match exprD' tus tvs t e' with
-                    | Some eD' =>
-                      SubstMorphism cs cs' /\
-                      (forall (us : hlist typD (getAmbientUVars ctx))
-                              (vs : hlist typD (getAmbientVars ctx)),
-                          csD'
-                            (fun (us0 : hlist typD (getUVars ctx))
-                                 (vs0 : hlist typD (getVars ctx)) =>
-                               rD (eD us0 vs0) (eD' us0 vs0)) us vs)
-                    | None => False
-                    end
-                  | None => False
-                  end
-                | None => True
-                end
-              | None => True
-              end).
-    Proof using RelDec_Correct_eq_typ RbaseD_single_type RTypeOk_typD RSymOk_func Typ2Ok_Fun tyArr.
-      Opaque vars_to_uvars.
-      unfold core_rewrite. generalize dependent 10.
-      simpl.
-      intros.
-      consider (typeof_expr nil l0.(vars) l0.(concl).(lhs)); intros.
-      { match goal with
-        | H : match ?X with _ => _ end = _ |- _ =>
-          consider X; intros
-        end; try match goal with
-                 | H : None = Some _ |- _ => exfalso ; clear - H ; inversion H
-                 end.
-        match goal with
-        | Hrt : rtacK_sound ?X , _ : match ?X _ _ _ _ ?C ?CS ?G with _ => _ end = _ |- _ =>
-          specialize (@Hrt C CS G _ eq_refl)
-        end.
-        match goal with
-        | Hrt : rtacK_spec _ _ ?X , H : match ?Y with _ => _ end = _ |- _ =>
-          replace Y with X in H ; [ generalize dependent X; intros | f_equal ]
-        end.
-        2: clear; simpl; repeat rewrite app_length; simpl; omega.
-        destruct r; try solve [ exfalso; clear - H4; inversion H4 ].
-        rewrite (ctx_subst_eta c0) in H4.
-        repeat match goal with
-               | H : match ?X with _ => _ end = _ |- _ =>
-                 let H' := fresh in
-                 destruct X eqn:H'; [ | solve [ exfalso; clear - H4; inversion H4 ] ]
-               end.
-        inv_all. subst.
-        destruct (@exprUnify_sound (ctx_subst (CExs ctx (vars l0))) typ func _ _ _ _ _ _ _ _ _ _ n
-                                   _ _ _ _ _ _ _ nil H3).
-        { constructor; eauto using WellFormed_entry_amap_empty. }
-        destruct H; eauto.
-        { eapply WellFormed_Goal_GConj_list.
-          induction (premises l0); simpl.
-          - constructor.
-          - constructor; eauto. constructor. }
-        split.
-        { rewrite ctx_subst_eta in H.
-          inv_all. assumption. }
-        intros.
-        destruct (pctxD cs) eqn:HpctxDcs; trivial.
-        destruct (exprD' (getUVars ctx) (getVars ctx) t0 e) eqn:HexprD'e; trivial.
-        simpl in *.
-        eapply lemmaD_lemmaD' in H0. forward_reason.
-        eapply lemmaD'_weakenU with (tus':=getUVars ctx) in H0;
-          eauto using ExprOk_expr, rw_concl_weaken.
-        simpl in H0. forward_reason.
-        unfold lemmaD' in H0.
-        forwardy. inv_all. subst.
-        unfold rw_conclD in H11.
-        forwardy. inv_all; subst.
-        assert (y1 = t).
-        { revert H11. revert H1. clear - RTypeOk_typD Typ2Ok_Fun RSymOk_func.
-          intros.
-          eapply ExprFacts.typeof_expr_weaken
-            with (tus':=getUVars ctx)
-                 (tvs':=nil)
-              in H1; eauto.
-          simpl in H1.
-          rewrite H1 in H11. inv_all. auto. }
-        subst t. rename y1 into t.
-        generalize (fun tus tvs e t => @ExprI.exprD'_conv typ _ (expr typ func)
-                                          _ tus tus (tvs ++ nil) tvs e t eq_refl
-                                          (eq_sym (app_nil_r_trans _))). simpl.
-        intro HexprD'_conv.
-        rewrite HexprD'_conv in H12. autorewrite_with_eq_rw_in H12.
-        rewrite HexprD'_conv in H13. autorewrite_with_eq_rw_in H13.
-        forwardy. inv_all. subst.
-
-        generalize (@vars_to_uvars_sound typ (expr typ func) _ _ _ _ _ _ _ _ nil _ _ _ H12).
-        simpl. destruct 1 as [ ? [ HexprD'e_subst ? ] ].
-        eapply exprD'_weakenV with (tvs':=getVars ctx) in HexprD'e_subst; eauto.
-        simpl in HexprD'e_subst. forward_reason.
-        assert (t = t0) by eauto using RD_single_type.
-        intros; subst.
-        replace (length (getUVars ctx ++ t0 :: nil))
-           with (S (length (getUVars ctx))) in H17
-             by (rewrite app_length; simpl; omega).
-        eapply exprD'_weakenU
-          with (tus':=l0.(vars)) in HexprD'e; eauto.
-        destruct (drop_exact_append_exact (vars l0) (getUVars ctx)) as [ ? [ Hx ? ] ].
-        rewrite Hx in *; clear Hx.
-        destruct (pctxD_substD H2 HpctxDcs) as [ ? [ Hx ? ] ].
-        rewrite Hx in *; clear Hx.
-        destruct HexprD'e as [ ? [ Hx ? ] ].
-        specialize (H6 _ _ _ H16 Hx eq_refl).
-        clear Hx.
-        forward_reason.
-        generalize (pctxD_SubstMorphism_progress H6).
-        simpl. rewrite HpctxDcs.
-        intro Hx; specialize (Hx _ eq_refl). destruct Hx.
-        rewrite H23 in *.
-        assert (exists Ps,
-                   goalD (getUVars ctx ++ vars l0) (getVars ctx)
-                         (GConj_list
-                            (map
-                               (fun e2 : expr typ func =>
-                                  GGoal (vars_to_uvars 0 (length (getUVars ctx)) e2))
-                               (premises l0))) = Some Ps /\
-                   forall (us : hlist typD (getUVars ctx)) us' vs,
-                     Ps (hlist_app us us') vs <->
-                     Forall (fun y => y us (hlist_app us' Hnil)) y).
-        { revert H0.
-          destruct l0. simpl in *.
-          clear - RTypeOk_typD RSymOk_func Typ2Ok_Fun.
-          intros.
-          cut (exists Ps : exprT (getUVars ctx ++ vars) (getVars ctx) Prop,
-                  goalD (getUVars ctx ++ vars) (getVars ctx)
-                        (GConj_list_simple
-                           (map
-                              (fun e2 : expr typ func =>
-                                 GGoal (vars_to_uvars 0 (length (getUVars ctx)) e2))
-                              premises)) = Some Ps /\
-                  (forall (us : hlist typD (getUVars ctx)) (us' : hlist typD vars)
-                          (vs : hlist typD (getVars ctx)),
-                      Ps (hlist_app us us') vs <->
-                      Forall
-                        (fun
-                            y0 : hlist typD (getUVars ctx) ->
-                                 hlist typD (vars ++ nil) -> Prop =>
-                            y0 us (hlist_app us' Hnil)) y)).
-          { destruct (goalD_GConj_list_GConj_list_simple
-                        (getUVars ctx ++ vars) (getVars ctx)
-                        (map (fun e2 : expr typ func =>
-                                GGoal (vars_to_uvars 0 (length (getUVars ctx)) e2))
-                           premises)).
-            { intros; forward_reason; congruence. }
-            { intros; forward_reason.
-              inv_all. subst. eexists; split; eauto.
-              intros.
-              rewrite <- H2. eapply H.
-              reflexivity. reflexivity. } }
-          revert H0. revert y.
-          induction premises; simpl; intros.
-          { eexists; split; eauto.
-            simpl. inv_all. subst.
-            split; eauto. }
-          { simpl in *.
-            forwardy. inv_all. subst.
-            unfold exprD'_typ0 in H.
-            simpl in H. forwardy.
-            generalize (@vars_to_uvars_sound typ (expr typ func) _ _ _ _ _ _ _ _ nil _ _ _ H).
-            intro. forward_reason.
-            unfold propD, exprD'_typ0.
-            simpl in H2.
-            eapply exprD'_weakenV
-              with (tvs':=getVars ctx)
-                in H2; eauto.
-            forward_reason. simpl in H2.
-            generalize (@exprD'_conv typ _ (expr typ func) _); eauto. simpl.
-            intro Hx.
-            rewrite Hx
-               with (pfu:=f_equal _ (eq_sym (app_nil_r_trans _))) (pfv:=eq_refl)
-                 in H2.
-            autorewrite_with_eq_rw_in H2.
-            forwardy.
-            rewrite H2.
-            specialize (IHpremises _ H0).
-            forward_reason. rewrite H6.
-            eexists; split; eauto. simpl.
-            intros.
-            inv_all. subst.
-            intros. rewrite Forall_cons_iff.
-            rewrite <- (H7 _ _ vs).
-            autorewrite with eq_rw.
-            specialize (H3 us (hlist_app us' Hnil) Hnil).
-            simpl in *.
-            rewrite H3; clear H3.
-            erewrite (H4 (hlist_app us (hlist_app us' Hnil)) Hnil vs); clear H4.
-            simpl. rewrite hlist_app_nil_r.
-            unfold f_equal.
-            autorewrite with eq_rw.
-            clear.
-            generalize (app_nil_r_trans vars).
-            generalize dependent (vars ++ nil).
-            intros; subst. reflexivity. } }
-        destruct H24 as [ ? [ Hx ? ] ].
-        rewrite Hx in *; clear Hx.
-        forwardy.
-        rewrite (ctx_subst_eta c0) in H7.
-        simpl in H7.
-        forwardy. rewrite H26.
-        inv_all; subst.
-        destruct (amap_substD_amap_empty (getUVars ctx ++ vars l0)
-                                         (getVars ctx)) as [ ? [ Hx ? ] ];
-          change_rewrite Hx in H6; clear Hx.
-        rewrite HpctxDcs in H6.
-        simpl in *.
-        destruct (drop_exact_append_exact l0.(vars) (getUVars ctx)) as [ ? [ Hx ? ] ];
-          rewrite Hx in *; clear Hx.
-        destruct H25.
-        inv_all. subst.
-        forwardy.
-        repeat match goal with
-               | H : ?X = _ , H' : ?X = _ |- _ => rewrite H in H'
-               end.
-        forward_reason; inv_all; subst.
-        simpl in *.
-        rewrite H7 in *.
-        rewrite H4 in *.
-        rewrite H6 in *.
-        rewrite H26 in *.
-        inv_all.
-        forwardy.
-        generalize H7. intro Hamap_substD.
-        eapply subst_getInstantiation in H7;
-          eauto using WellFormed_entry_WellFormed_pre_entry
-                 with typeclass_instances.
-        destruct H7.
-        assert (exists e'D,
-                   exprD' (getUVars ctx) (getVars ctx) t0
-                          (instantiate (fun u : ExprI.uvar => amap_lookup u x12)
-                                       0 (vars_to_uvars 0 (length (getUVars ctx)) l0.(concl).(rhs))) = Some e'D /\
-                   forall us vs,
-                     e'D us vs =
-                     y0 us (hlist_map
-                              (fun (t : typ) (x6 : exprT (getUVars ctx) (getVars ctx) (typD t)) =>
-                                 x6 us vs) x5)).
-        { (** this says that I can strengthen the expression **)
-          (** TODO: This should be a lemma **)
-          revert H13. revert H. revert H5. revert Hamap_substD.
-          clear - RTypeOk_typD RSymOk_func Typ2Ok_Fun H40.
-(*          remember (getUVars ctx). *)
-          generalize dependent (getVars ctx).
-          generalize dependent (rhs (concl l0)).
-          generalize dependent (vars l0).
-          clear - RTypeOk_typD RSymOk_func Typ2Ok_Fun.
-          intros.
-          generalize (@vars_to_uvars_sound typ (expr typ func) _ _ _ _ _ _ _ e nil t0 l _ H13).
-          destruct 1 as [ ? [ ? ? ] ].
-          eapply ExprI.exprD'_weakenV with (tvs':=t) in H0; eauto with typeclass_instances.
-          destruct H0 as [ ? [ ? ? ] ].
-          destruct (@instantiate_sound typ (expr typ func) _ _ _ (getUVars ctx++l) t
-                                       (fun u : ExprI.uvar => amap_lookup u x12)
-                                       (vars_to_uvars 0 (length (getUVars ctx)) e) nil t0 x0 y3).
-          { generalize (@sem_preserves_if_substD (amap (expr typ func)) typ (expr typ func) _ _ _ _).
-            simpl. intro. eapply H3.
-            2: eapply Hamap_substD.
-            eapply WellFormed_entry_WellFormed_pre_entry in H40.
-            destruct H40. assumption. }
-          { eassumption. }
-          { destruct H3.
-            eapply exprD'_strengthenU_multi in H3.
-            2: eauto with typeclass_instances.
-            { destruct H3 as [ ? [ ? ? ] ].
-              eexists; split; try eassumption.
-              intros.
-              specialize (H us vs).
-              specialize (H4 _ _ Hnil H).
-              simpl in *.
-              symmetry.
-              etransitivity; [ eapply (H1 _ _ Hnil) | ].
-              etransitivity; [ eapply H2 | ].
-              etransitivity; [ eapply H4 | ].
-              eapply H6. }
-            { intros.
-              clear H2 H1 H3 H4 H.
-              match goal with
-              | |- ?X = _ => consider X; try reflexivity; intro
-              end.
-              exfalso.
-              eapply mentionsU_instantiate in H.
-              assert (amap_lookup (length (getUVars ctx) + u) x12 <> None).
-              { clear - H5 H40 H6.
-                destruct H40.
-                clear H0.
-                red in H.
-                destruct H as [ ? [ ? ? ] ].
-                clear H H1.
-                generalize dependent (length (getUVars ctx)).
-                generalize dependent (length l).
-                clear.
-                intros.
-                eapply pigeon_principle; eauto. }
-              destruct H.
-              { destruct H. eauto. }
-              { destruct H. destruct H. destruct H as [ ? [ ? ? ] ].
-                destruct H40.
-                consider (amap_lookup (length (getUVars ctx) + u) x12); intros; try congruence.
-                eapply FMapSubst.SUBST.normalized_fmapsubst in H1.
-                3: eapply H.
-                cut (true = false); [ clear; intros; congruence | ].
-                rewrite <- H3. rewrite <- H1. reflexivity.
-                destruct H4. assumption. } } } }
-        destruct H7 as [ ? [ Hx ? ] ]; rewrite Hx; clear Hx.
-        split.
-        { etransitivity; eassumption. }
-        intros.
-        eapply pctxD_substD' with (us:=us) (vs:=vs) in H37; eauto with typeclass_instances.
-        gather_facts.
-        eapply pctxD_SubstMorphism; [ | | eauto | ]; eauto.
-        gather_facts.
-        eapply pctxD_SubstMorphism; [ | | eauto | ]; eauto.
-        gather_facts.
-        eapply Pure_pctxD; eauto. intros.
-        specialize (H us0 vs0).
-        specialize (H7 us0 vs0).
-        generalize dependent (hlist_map
-           (fun (t : typ) (x6 : exprT (getUVars ctx) (getVars ctx) (typD t)) =>
-            x6 us0 vs0) x5); simpl; intros.
-        apply (H10 _ us0 _) in H9; clear H10.
-        rewrite foralls_sem in H9.
-        setoid_rewrite impls_sem in H9.
-        generalize (H9 h); clear H9.
-        rewrite Quant._forall_sem in H25.
-        simpl.
-        specialize (H25 _ H).
-        specialize (H23 _ H).
-        specialize (H21 _ H23).
-        rewrite H7; clear H7.
-        rewrite (H20 us0 vs0 h); clear H20.
-        specialize (H22 (hlist_app us0 h) vs0).
-        rewrite H28 in H22.
-        specialize (H22 (conj H23 H19)).
-        forward_reason.
-        specialize (H9 Hnil).
-        simpl in H9.
-        rewrite <- H9; clear H9.
-        specialize (fun X => H17 X Hnil); simpl in H17.
-        rewrite <- H17; clear H17.
-        rewrite <- H15; clear H15.
-        rewrite hlist_app_nil_r.
-        autorewrite with eq_rw.
-        simpl.
-        refine (fun x => x _).
-        clear x14.
-        eapply List.Forall_map.
-        eapply H24 in H25.
-        revert H25.
-        eapply Forall_impl.
-        intro. rewrite hlist_app_nil_r. tauto. }
-      { exfalso; clear - H3; inversion H3. }
-    Time Qed.
-
-    Theorem using_rewrite_db'_sound
-    : forall r ctx (cs : ctx_subst ctx),
-        let tus := getUVars ctx in
-        let tvs := getVars ctx in
-        forall hints : list (rw_lemma typ func Rbase * rtacK typ (expr typ func)),
-        Forall (fun lt =>
-                  lemmaD (rw_conclD RbaseD) nil nil (fst lt) /\
-                  rtacK_sound (snd lt)) hints ->
-        forall e e' cs',
-          @using_rewrite_db' hints e r tus tvs (length tus) (length tvs) ctx cs = Some (e', cs') ->
-          WellFormed_ctx_subst cs ->
-          WellFormed_ctx_subst cs' /\
-          (forall (t : typ) (rD : typD t -> typD t -> Prop),
-              RD RbaseD r t = Some rD ->
-              match pctxD cs with
-              | Some _ =>
-                match exprD' tus tvs t e with
-                | Some eD =>
-                  match pctxD cs' with
-                  | Some csD' =>
-                    match exprD' tus tvs t e' with
-                    | Some eD' =>
-                      SubstMorphism cs cs' /\
-                      (forall (us : hlist typD (getAmbientUVars ctx))
-                              (vs : hlist typD (getAmbientVars ctx)),
-                          csD'
-                            (fun (us0 : hlist typD (getUVars ctx))
-                                 (vs0 : hlist typD (getVars ctx)) =>
-                                 rD (eD us0 vs0)
-                                    (eD' us0 vs0)) us vs)
-                    | None => False
-                    end
-                  | None => False
-                  end
-                | None => True
-                end
-              | None => True
-              end).
-    Proof.
-      clear transitiveOk reflexiveOk respectfulOk rwOk.
-      clear rw respectful transitive reflexive.
-      induction 1.
-      { simpl. inversion 1. }
-      { simpl. intros. destruct x.
-        assert (using_rewrite_db' l e r tus tvs (length tus) (length tvs) cs = Some (e',cs')
-             \/ (r = l0.(concl).(rel) /\
-                 core_rewrite l0 r0 e tus tvs (length tus) (length tvs) cs = Some (e',cs'))).
-        { generalize (Req_dec_ok Rbase_eq Rbase_eq_ok r l0.(concl).(rel)).
-          destruct (Req_dec Rbase_eq r l0.(concl).(rel)); eauto.
-          intros. destruct (core_rewrite l0 r0 e tus tvs (length tus) (length tvs) cs); eauto. }
-        clear H1. destruct H3; eauto.
-        destruct H1. subst. clear IHForall H0.
-        simpl in H. destruct H.
-        revert H2. revert H3. revert H. revert H0.
-        intros.
-        eapply core_rewrite_sound in H3; eauto. }
-    Qed.
-
-    Lemma SubstMorphism_wrap_tvs_ctx_subst
-      : forall tvs' ctx cs c,
-        SubstMorphism (wrap_tvs_ctx_subst tvs' cs) c ->
-        SubstMorphism cs
-                      (unwrap_tvs_ctx_subst tvs' c (fun x : ctx_subst ctx => x)).
-    Proof.
-      clear. intros.
-      rewrite <- unwrap_tvs_ctx_subst_unwrap_tvs_ctx_subst'.
-      revert H. revert ctx c cs.
-      induction tvs'.
-      { simpl. tauto. }
-      { simpl. intros.
-        eapply IHtvs' in H.
-        inv_all. rewrite H. assumption. }
-    Qed.
-
-    Theorem using_rewrite_db_sound
-    : forall hints : list (rw_lemma typ func Rbase * rtacK typ (expr typ func)),
-        Forall (fun lt =>
-                  lemmaD (rw_conclD RbaseD) nil nil (fst lt) /\
-                  rtacK_sound (snd lt)) hints ->
-        setoid_rewrite_spec (fun e r =>
-                               rw_bind (using_rewrite_db hints e r)
-                                       (fun e => rw_ret (Progress e))).
-    Proof.
-      clear transitiveOk reflexiveOk respectfulOk rwOk.
-      clear rw respectful transitive reflexive.
-      unfold using_rewrite_db.
-      unfold for_tactic.
-      red. red. intros.
-      unfold rw_bind in H0.
-      forwardy. inv_all. subst.
-      rewrite Plus.plus_comm in H0. rewrite <- app_length in H0.
-      destruct (fun Hx =>
-                    @using_rewrite_db'_sound r _ (wrap_tvs_ctx_subst tvs' cs) hints H
-                                             (expr_convert (length tvs') (length (getVars ctx)) e) e1 c0 Hx
-                                             (WellFormed_ctx_subst_wrap_tvs _ H1)).
-      { rewrite <- H0. f_equal.
-        eauto using getUVars_wrap_tvs.
-        eauto using getVars_wrap_tvs.
-        rewrite getUVars_wrap_tvs. reflexivity.
-        rewrite getVars_wrap_tvs. reflexivity. }
-      clear H0. subst.
-      split.
-      { eapply WellFormed_ctx_subst_unwrap_tvs
-          with (ctx':=CTop nil nil); eauto. }
-      intros.
-      specialize (H3 _ _ H0); clear H0.
-      destruct (pctxD cs) eqn:HpctxD_cs; trivial.
-      destruct (@pctxD_wrap_tvs_ctx_subst tvs' _ _ _ HpctxD_cs) as [ ? [ ? ? ] ].
-      rewrite H0 in H3.
-      destruct (exprD' (getUVars ctx) (tvs' ++ getVars ctx) t e) eqn:HexprD'_e; trivial.
-      generalize (@exprD'_conv typ _ (expr typ func) _). simpl.
-      intro Hconv.
-      rewrite Hconv
-         with (tus':=getUVars ctx) (tvs':=getVars ctx++tvs')
-              (pfu:=eq_sym (getUVars_wrap_tvs tvs' ctx)) (pfv:=eq_sym (getVars_wrap_tvs tvs' ctx))
-           in H3.
-      clear Hconv.
-      eapply expr_convert_sound in HexprD'_e.
-      destruct HexprD'_e as [ ? [ Hx ? ] ].
-      rewrite Hx in *; clear Hx.
-      autorewrite_with_eq_rw_in H3.
-      forwardy.
-      destruct (pctxD_unwrap_tvs_ctx_subst _ _ _ H3) as [ ? [ HpctxD_x1 ? ] ].
-      rewrite HpctxD_x1.
-      generalize (@exprD'_conv typ _ (expr typ func) _). simpl.
-      intro Hconv.
-      rewrite Hconv
-         with (pfu:=eq_sym (getUVars_wrap_tvs tvs' ctx)) (pfv:=eq_sym(getVars_wrap_tvs tvs' ctx))
-           in H6.
-      clear Hconv.
-      autorewrite_with_eq_rw_in H6.
-      forwardy; inv_all; subst.
-      eapply expr_convert_sound in H6.
-      destruct H6 as [ ? [ Hx ? ] ]; rewrite Hx; clear Hx.
-      destruct H7.
-      split.
-      { clear H9 H8 H4.
-        eapply SubstMorphism_wrap_tvs_ctx_subst; eauto. }
-      { intros.
-        specialize (H9 match
-                        eq_sym (getAmbientUVars_wrap_tvs tvs' ctx) in (_ = V)
-                        return (hlist typD V)
-                      with
-                      | eq_refl => us
-                      end
-                       match
-                         eq_sym (getAmbientVars_wrap_tvs tvs' ctx) in (_ = V)
-                         return (hlist typD V)
-                       with
-                       | eq_refl => vs
-                       end).
-        specialize (H8 us vs
-                   (fun us0 vs0 =>
-                      rD (x0 us0 vs0) (y2 us0 vs0))).
-        simpl in H8.
-        generalize dependent (getVars_wrap_tvs tvs' ctx).
-        generalize dependent (getUVars_wrap_tvs tvs' ctx).
-        generalize dependent (getAmbientUVars_wrap_tvs tvs' ctx).
-        generalize dependent (getAmbientVars_wrap_tvs tvs' ctx).
-        generalize (Ap_pctxD _ HpctxD_x1).
-        generalize (Pure_pctxD _ HpctxD_x1).
-        revert H5 H6 H7. clear.
-        generalize dependent (getAmbientVars (wrap_tvs tvs' ctx)).
-        generalize dependent (getAmbientUVars (wrap_tvs tvs' ctx)).
-        generalize dependent (getUVars (wrap_tvs tvs' ctx)).
-        generalize dependent (getVars (wrap_tvs tvs' ctx)).
-        intros; subst; simpl in *.
-        eapply H8 in H9; clear H8.
-        revert H9. eapply H0; clear H0.
-        eapply H; clear H.
-        clear - H5 H6.
-        intros. rewrite H5. rewrite <- H6. eauto. }
-    Time Qed.
-
-    (** TODO(gmalecha): This is almost identical to the above theorem *)
-    Theorem using_prewrite_db_sound
-    : forall hints : expr typ func ->
-                     list (rw_lemma typ func Rbase * rtacK typ (expr typ func)),
-        (forall e, Forall (fun lt =>
-                             lemmaD (rw_conclD RbaseD) nil nil (fst lt) /\
-                             rtacK_sound (snd lt)) (hints e)) ->
-        setoid_rewrite_spec (fun e r =>
-                               rw_bind (using_prewrite_db hints e r)
-                                       (fun e => rw_ret (Progress e))).
-    Proof.
-      intros.
-      clear transitiveOk reflexiveOk respectfulOk rwOk.
-      clear rw respectful transitive reflexive.
-      unfold using_prewrite_db.
-      unfold for_tactic.
-      red. red. intros.
-      unfold rw_bind in H0.
-      forwardy. inv_all. subst.
-      rewrite Plus.plus_comm in H0. rewrite <- app_length in H0.
-      destruct (fun Hx =>
-                    @using_rewrite_db'_sound r _ (wrap_tvs_ctx_subst tvs' cs)
-                                             (hints (expr_convert (length tvs') (length (getVars ctx)) e)) (H _)
-                                             (expr_convert (length tvs') (length (getVars ctx)) e) e1 c0 Hx
-                                             (WellFormed_ctx_subst_wrap_tvs _ H1)).
-      { rewrite <- H0. f_equal.
-        eauto using getUVars_wrap_tvs.
-        eauto using getVars_wrap_tvs.
-        rewrite getUVars_wrap_tvs. reflexivity.
-        rewrite getVars_wrap_tvs. reflexivity. }
-      clear H0. subst.
-      split.
-      { eapply WellFormed_ctx_subst_unwrap_tvs
-          with (ctx':=CTop nil nil); eauto. }
-      intros.
-      specialize (H3 _ _ H0); clear H0.
-      destruct (pctxD cs) eqn:HpctxD_cs; trivial.
-      destruct (@pctxD_wrap_tvs_ctx_subst tvs' _ _ _ HpctxD_cs) as [ ? [ ? ? ] ].
-      rewrite H0 in H3.
-      destruct (exprD' (getUVars ctx) (tvs' ++ getVars ctx) t e) eqn:HexprD'_e; trivial.
-      generalize (@exprD'_conv typ _ (expr typ func) _). simpl.
-      intro Hconv.
-      rewrite Hconv
-         with (tus':=getUVars ctx) (tvs':=getVars ctx++tvs')
-              (pfu:=eq_sym (getUVars_wrap_tvs tvs' ctx)) (pfv:=eq_sym (getVars_wrap_tvs tvs' ctx))
-           in H3.
-      clear Hconv.
-      eapply expr_convert_sound in HexprD'_e.
-      destruct HexprD'_e as [ ? [ Hx ? ] ].
-      rewrite Hx in *; clear Hx.
-      autorewrite_with_eq_rw_in H3.
-      forwardy.
-      destruct (pctxD_unwrap_tvs_ctx_subst _ _ _ H3) as [ ? [ HpctxD_x1 ? ] ].
-      rewrite HpctxD_x1.
-      generalize (@exprD'_conv typ _ (expr typ func) _). simpl.
-      intro Hconv.
-      rewrite Hconv
-         with (pfu:=eq_sym (getUVars_wrap_tvs tvs' ctx)) (pfv:=eq_sym(getVars_wrap_tvs tvs' ctx))
-           in H6.
-      clear Hconv.
-      autorewrite_with_eq_rw_in H6.
-      forwardy; inv_all; subst.
-      eapply expr_convert_sound in H6.
-      destruct H6 as [ ? [ Hx ? ] ]; rewrite Hx; clear Hx.
-      destruct H7.
-      split.
-      { clear H9 H8 H4.
-        eapply SubstMorphism_wrap_tvs_ctx_subst; eauto. }
-      { intros.
-        specialize (H9 match
-                        eq_sym (getAmbientUVars_wrap_tvs tvs' ctx) in (_ = V)
-                        return (hlist typD V)
-                      with
-                      | eq_refl => us
-                      end
-                       match
-                         eq_sym (getAmbientVars_wrap_tvs tvs' ctx) in (_ = V)
-                         return (hlist typD V)
-                       with
-                       | eq_refl => vs
-                       end).
-        specialize (H8 us vs
-                   (fun us0 vs0 =>
-                      rD (x0 us0 vs0) (y2 us0 vs0))).
-        simpl in H8.
-        generalize dependent (getVars_wrap_tvs tvs' ctx).
-        generalize dependent (getUVars_wrap_tvs tvs' ctx).
-        generalize dependent (getAmbientUVars_wrap_tvs tvs' ctx).
-        generalize dependent (getAmbientVars_wrap_tvs tvs' ctx).
-        generalize (Ap_pctxD _ HpctxD_x1).
-        generalize (Pure_pctxD _ HpctxD_x1).
-        revert H5 H6 H7. clear.
-        generalize dependent (getAmbientVars (wrap_tvs tvs' ctx)).
-        generalize dependent (getAmbientUVars (wrap_tvs tvs' ctx)).
-        generalize dependent (getUVars (wrap_tvs tvs' ctx)).
-        generalize dependent (getVars (wrap_tvs tvs' ctx)).
-        intros; subst; simpl in *.
-        eapply H8 in H9; clear H8.
-        revert H9. eapply H0; clear H0.
-        eapply H; clear H.
-        clear - H5 H6.
-        intros. rewrite H5. rewrite <- H6. eauto. }
-    Qed.
-
-    Instance Injective_mrw_equiv_rw_ret {T} (rT : T -> T -> Prop) (a b : T)
-    : Injective (mrw_equiv rT (rw_ret a) (rw_ret b)) :=
-    { result := rT a b }.
-    Proof.
-      unfold rw_ret. clear. intros. red in H.
-      specialize (H nil nil nil 0 0 _ (@TopSubst _ _ nil nil)).
-      inv_all. assumption.
-    Defined.
-
-    Definition rw_bind_catch {T U : Type} (c : mrw T) (k : T -> mrw U)
-               (otherwise : mrw U)
-    : mrw U :=
-      fun tus' tus tvs nus nvs ctx cs =>
-        match c tus' tus tvs nus nvs ctx cs with
-        | None => otherwise tus' tus tvs nus nvs ctx cs
-        | Some (val,cs') => k val tus' tus tvs nus nvs ctx cs'
-        end.
-
-    Lemma rw_orelse_case
-      : forall (T : Type) (A B : mrw T) a b c d e f g h,
-        @rw_orelse _ A B a b c d e f g = h ->
-        A a b c d e f g = h \/
-        B a b c d e f g = h.
-    Proof.
-      clear. unfold rw_orelse. intros.
-      forward.
-    Qed.
-
-    Lemma rw_bind_catch_case
-      : forall (T U : Type) (A : mrw T) (B : T -> mrw U) (C : mrw U)
-               a b c d e f g h,
-        @rw_bind_catch _ _ A B C a b c d e f g = h ->
-        (exists x g', A a b c d e f g = Some (x,g') /\
-                      B x a b c d e f g' = h) \/
-        (C a b c d e f g = h /\ A a b c d e f g = None).
-    Proof. clear.
-           unfold rw_bind_catch. intros; forward.
-           left. do 2 eexists; split; eauto.
-    Qed.
-
-    Lemma rw_bind_case
-      : forall (T U : Type) (A : mrw T) (B : T -> mrw U)
-               a b c d e f g h,
-        @rw_bind _ _ A B a b c d e f g = Some h ->
-        exists x g',
-          A a b c d e f g = Some (x, g') /\
-          B x a b c d e f g' = Some h.
-    Proof. clear.
-           unfold rw_bind. intros; forward.
-           do 2 eexists; eauto.
-    Qed.
 
     Lemma RD_tyAcc : forall d a b c e f,
         RD RbaseD a b = Some c ->
@@ -2052,8 +778,6 @@ Section setoid.
         { exfalso. clear - H5. inversion H5. } }
     Time Qed.
 
-
-
     Theorem recursive_rewrite_sound
     : forall tvs',
         forall es ctx (cs : ctx_subst ctx) cs' f f' rs e',
@@ -2173,6 +897,7 @@ Section setoid.
               else rw_fail))
         e r.
 *)
+
     Lemma bottom_up_sound_lem
     : forall e rg,
         @setoid_rewrite_rel e rg (bottom_up e rg).
@@ -2212,7 +937,7 @@ Section setoid.
                 destruct (exprD' (getUVars ctx) (tvs' ++ getVars ctx) t (apps e (map fst es)))
                          eqn:HexprD'apps_e_es; trivial.
                 specialize (fun ts fD rD => H5 _ _ _ H8 ts fD rD _ HexprD'apps_e_es).
-                eapply apps_exprD'_fold_type in HexprD'apps_e_es.
+                eapply apps_exprD'_fold_type in HexprD'apps_e_es; eauto.
                 forward_reason.
                 specialize (H4 x4).
                 rewrite H9 in H4.
@@ -2259,7 +984,7 @@ Section setoid.
                 destruct (exprD' (getUVars ctx) (tvs' ++ getVars ctx) t
                                  (apps e (map fst es))) eqn:HexprD'_e; trivial.
                 specialize (fun ts fD rD => H5 ts fD rD _ eq_refl).
-                eapply apps_exprD'_fold_type in HexprD'_e.
+                eapply apps_exprD'_fold_type in HexprD'_e; try assumption.
                 forward_reason.
                 specialize (H4 x1).
                 rewrite H7 in H4.
@@ -2293,7 +1018,7 @@ Section setoid.
                 destruct (exprD' (getUVars ctx) (tvs' ++ getVars ctx) t (apps e (map fst es))) eqn:HexprD'apps_e_es; trivial.
                 specialize (H5 _ _ _ H8).
                 rewrite HexprD'apps_e_es in H5.
-                eapply apps_exprD'_fold_type in HexprD'apps_e_es.
+                eapply apps_exprD'_fold_type in HexprD'apps_e_es; try assumption.
                 forward_reason.
                 specialize (H4 x1).
                 generalize (H5 x1); clear H5.
@@ -2318,7 +1043,7 @@ Section setoid.
                 specialize (fun ts => H4 ts _ _ H6); specialize (H5 _ _ _ H6).
                 destruct (pctxD cs) eqn:pctxD_cs; trivial.
                 destruct (exprD' (getUVars ctx) (tvs' ++ getVars ctx) t (apps e (map fst es))) eqn:HexprD'apps_e_es; trivial.
-                eapply apps_exprD'_fold_type in HexprD'apps_e_es.
+                eapply apps_exprD'_fold_type in HexprD'apps_e_es; try assumption.
                 forward_reason.
                 specialize (H4 x1).
                 generalize (H5 x1); clear H5.
@@ -2346,7 +1071,7 @@ Section setoid.
               specialize (fun ts => H4 ts _ _ H3).
               destruct (pctxD cs) eqn:HpctxDcs; trivial.
               destruct (exprD' (getUVars ctx) (tvs' ++ getVars ctx) t (apps e (map fst es))) eqn:HexprD'apps_e_es; trivial.
-              destruct (apps_exprD'_fold_type _ _ _ HexprD'apps_e_es).
+              destruct (apps_exprD'_fold_type _ _ _ _ _ _ HexprD'apps_e_es).
               forward_reason.
               specialize (H4 x1).
               specialize (fun rD => H5 x1 _ rD _ eq_refl H6).
@@ -2376,7 +1101,7 @@ Section setoid.
               destruct (exprD' (getUVars ctx) (tvs' ++ getVars ctx) t
                                (apps e (map fst es)))
                        eqn:HexprD'_apps_e_es; trivial.
-              destruct (apps_exprD'_fold_type _ _ _ HexprD'_apps_e_es).
+              destruct (apps_exprD'_fold_type _ _ _ _ _ _ HexprD'_apps_e_es).
               forward_reason.
               specialize (H4 x1).
               rewrite H8 in *.
@@ -2443,6 +1168,10 @@ Section setoid.
         e nil r.
 *)
   End top_bottom.
+
+
+  (** This should probably go somewhere else **)
+  Section the_tactic.
 
   Definition auto_setoid_rewrite_bu
              (r : R)
@@ -2523,9 +1252,1455 @@ Section setoid.
       eapply rtac_spec_Fail. }
   Qed.
 
+  End the_tactic.
+
+  (** This starts plugins for the rewriter **)
+  (******************************************)
+
+  Definition func_sdec (a b : func) : bool :=
+    match sym_eqb a b with
+    | Some x => x
+    | _ => false
+    end.
+
+  Definition expr_sdec : expr typ func -> expr typ func -> bool :=
+    @expr_eq_sdec typ func _ func_sdec.
+
+  Lemma expr_sdec_sound
+  : forall a b : expr typ func, expr_sdec a b = true -> a = b.
+  Proof.
+    eapply expr_eq_sdec_ok; eauto.
+    unfold func_sdec.
+    intros. generalize (sym_eqbOk a b); eauto with typeclass_instances.
+    destruct (sym_eqb a b); intros; subst; auto.
+    inversion H.
+  Qed.
+
+  Section core_rewrite.
+    (* This is the implementation of rewriting a single lemma *)
+    (** Note, this is quite inefficient due to building and destructing
+     ** the pair
+     **)
+    Fixpoint extend_ctx (tvs' : tenv typ)
+             (ctx : Ctx typ (expr typ func)) (cs : ctx_subst ctx) {struct tvs'}
+    : { ctx : Ctx typ (expr typ func) & ctx_subst ctx } :=
+      match tvs' with
+      | nil => @existT _ _ ctx cs
+      | t :: tvs' =>
+        match @extend_ctx tvs' ctx cs with
+        | existT _ ctx' cs' => @existT _ _ (CAll ctx' t) (AllSubst cs')
+        end
+      end.
+
+    (** TODO(gmalecha): This is not a nice interface because it is not
+     ** a standard rewriter for two reasons:
+     ** 1) It assumes that tvs' = nil, and
+     ** 2) It assumes that the relation is the same as the relation for
+     **    the lemma.
+     **)
+    Definition core_rewrite (lem : rw_lemma typ func Rbase)
+               (tac : rtacK typ (expr typ func))
+    : expr typ func -> tenv typ -> tenv typ -> nat -> nat ->
+      forall c : Ctx typ (expr typ func),
+        ctx_subst c -> option (expr typ func * ctx_subst c) :=
+        match typeof_expr nil lem.(vars) lem.(concl).(lhs) with
+        | None => fun _ _ _ _ _ _ _ => None
+        | Some t =>
+          fun e tus tvs nus nvs ctx cs =>
+           let ctx' := CExs ctx lem.(vars) in
+           let cs' : ctx_subst ctx' := ExsSubst cs (amap_empty _) in
+           let tus' := tus ++ lem.(vars) in
+           match
+             exprUnify 10 tus' tvs 0 (vars_to_uvars 0 nus lem.(concl).(lhs))
+                       e t cs'
+           with
+           | None => None
+           | Some cs'' =>
+             let prems :=
+                 List.map (fun e => GGoal (vars_to_uvars 0 nus e)) lem.(premises)
+             in
+             match
+               tac tus' tvs (length lem.(vars) + nus) nvs ctx' cs'' (GConj_list prems)
+             with
+             | Solved cs''' =>
+               match cs''' in ctx_subst ctx
+                     return match ctx with
+                            | CExs z _ => option (expr typ func * ctx_subst z)
+                            | _ => unit
+                            end
+               with
+               | ExsSubst cs'''' sub =>
+		 if amap_is_full (length lem.(vars)) sub then
+                   let res :=
+                       instantiate (fun u => amap_lookup u sub) 0
+                                   (vars_to_uvars 0 nus lem.(concl).(rhs))
+                   in
+                   Some (res, cs'''')
+                 else
+                   None
+               | _ => tt
+               end
+             | _ => None
+             end
+           end
+        end.
+
+    (** TODO: Move **)
+    Lemma exprD'_weakenV
+    : forall (tus tvs : tenv typ) (e : expr typ func) (t : typ)
+             (val : exprT tus tvs (typD t)) (tvs' : list typ),
+        exprD' tus tvs t e = Some val ->
+        exists val' : exprT tus (tvs ++ tvs') (typD t),
+          exprD' tus (tvs ++ tvs') t e = Some val' /\
+          (forall (us : hlist typD tus) (vs : hlist typD tvs)
+                  (vs' : hlist typD tvs'),
+              val us vs = val' us (hlist_app vs vs')).
+    Proof.
+      intros.
+      generalize (@exprD'_weakenV typ _ (expr typ func) _ _ tus tvs tvs' e t val H).
+      eauto.
+    Qed.
+
+    (** TODO: Move **)
+    Lemma exprD'_weakenU
+    : forall (tus tvs : tenv typ) (e : expr typ func) (t : typ)
+             (val : exprT tus tvs (typD t)) (tus' : list typ),
+        exprD' tus tvs t e = Some val ->
+        exists val' : exprT (tus ++ tus') tvs (typD t),
+          exprD' (tus ++ tus') tvs t e = Some val' /\
+          (forall (us : hlist typD tus) (vs : hlist typD tvs)
+                  (us' : hlist typD tus'),
+              val us vs = val' (hlist_app us us') vs).
+    Proof.
+      intros.
+      generalize (@exprD'_weakenU typ _ (expr typ func) _ _ tus tus' tvs e t val H).
+      eauto.
+    Qed.
+
+    Local Instance Subst_amap T : Subst (amap T) T :=
+      FMapSubst.SUBST.Subst_subst T.
+    Local Instance SubstOk_amap : SubstOk (Subst_amap (expr typ func)) :=
+      @FMapSubst.SUBST.SubstOk_subst typ _ (expr typ func) _.
+
+    Opaque instantiate.
+
+    (* TODO(gmalecha): This is not a nice interface! *)
+    Theorem core_rewrite_sound
+    : forall ctx (cs : ctx_subst ctx),
+        let tus := getUVars ctx in
+        let tvs := getVars ctx in
+        forall l0 r0 e e' cs',
+          rtacK_sound r0 ->
+          lemmaD (rw_conclD RbaseD) nil nil l0 ->
+          core_rewrite l0 r0 e tus tvs (length tus) (length tvs) cs = Some (e', cs') ->
+          WellFormed_ctx_subst cs ->
+          WellFormed_ctx_subst cs' /\
+          (forall (t : typ) (rD : typD t -> typD t -> Prop),
+              RD RbaseD (rel (concl l0)) t = Some rD ->
+              match pctxD cs with
+              | Some _ =>
+                match exprD' tus tvs t e with
+                | Some eD =>
+                  match pctxD cs' with
+                  | Some csD' =>
+                    match exprD' tus tvs t e' with
+                    | Some eD' =>
+                      SubstMorphism cs cs' /\
+                      (forall (us : hlist typD (getAmbientUVars ctx))
+                              (vs : hlist typD (getAmbientVars ctx)),
+                          csD'
+                            (fun (us0 : hlist typD (getUVars ctx))
+                                 (vs0 : hlist typD (getVars ctx)) =>
+                               rD (eD us0 vs0) (eD' us0 vs0)) us vs)
+                    | None => False
+                    end
+                  | None => False
+                  end
+                | None => True
+                end
+              | None => True
+              end).
+    Proof using RelDec_Correct_eq_typ RbaseD_single_type
+          RTypeOk_typD RSymOk_func Typ2Ok_Fun tyArr.
+      Opaque vars_to_uvars.
+      unfold core_rewrite. generalize dependent 10.
+      simpl.
+      intros.
+      consider (typeof_expr nil l0.(vars) l0.(concl).(lhs)); intros.
+      { match goal with
+        | H : match ?X with _ => _ end = _ |- _ =>
+          consider X; intros
+        end; try match goal with
+                 | H : None = Some _ |- _ => exfalso ; clear - H ; inversion H
+                 end.
+        match goal with
+        | Hrt : rtacK_sound ?X , _ : match ?X _ _ _ _ ?C ?CS ?G with _ => _ end = _ |- _ =>
+          specialize (@Hrt C CS G _ eq_refl)
+        end.
+        match goal with
+        | Hrt : rtacK_spec _ _ ?X , H : match ?Y with _ => _ end = _ |- _ =>
+          replace Y with X in H ; [ generalize dependent X; intros | f_equal ]
+        end.
+        2: clear; simpl; repeat rewrite app_length; simpl; omega.
+        destruct r; try solve [ exfalso; clear - H4; inversion H4 ].
+        rewrite (ctx_subst_eta c0) in H4.
+        repeat match goal with
+               | H : match ?X with _ => _ end = _ |- _ =>
+                 let H' := fresh in
+                 destruct X eqn:H'; [ | solve [ exfalso; clear - H4; inversion H4 ] ]
+               end.
+        inv_all. subst.
+        destruct (@exprUnify_sound (ctx_subst (CExs ctx (vars l0))) typ func _ _ _ _ _ _ _ _ _ _ n
+                                   _ _ _ _ _ _ _ nil H3).
+        { constructor; eauto using WellFormed_entry_amap_empty. }
+        destruct H; eauto.
+        { eapply WellFormed_Goal_GConj_list.
+          induction (premises l0); simpl.
+          - constructor.
+          - constructor; eauto. constructor. }
+        split.
+        { rewrite ctx_subst_eta in H.
+          inv_all. assumption. }
+        intros.
+        destruct (pctxD cs) eqn:HpctxDcs; trivial.
+        destruct (exprD' (getUVars ctx) (getVars ctx) t0 e) eqn:HexprD'e; trivial.
+        simpl in *.
+        eapply lemmaD_lemmaD' in H0. forward_reason.
+        eapply lemmaD'_weakenU with (tus':=getUVars ctx) in H0;
+          eauto using ExprOk_expr, rw_concl_weaken.
+        simpl in H0. forward_reason.
+        unfold lemmaD' in H0.
+        forwardy. inv_all. subst.
+        unfold rw_conclD in H11.
+        forwardy. inv_all; subst.
+        assert (y1 = t).
+        { revert H11. revert H1. clear - RTypeOk_typD Typ2Ok_Fun RSymOk_func.
+          intros.
+          eapply ExprFacts.typeof_expr_weaken
+            with (tus':=getUVars ctx)
+                 (tvs':=nil)
+              in H1; eauto.
+          simpl in H1.
+          rewrite H1 in H11. inv_all. auto. }
+        subst t. rename y1 into t.
+        generalize (fun tus tvs e t => @ExprI.exprD'_conv typ _ (expr typ func)
+                                          _ tus tus (tvs ++ nil) tvs e t eq_refl
+                                          (eq_sym (app_nil_r_trans _))). simpl.
+        intro HexprD'_conv.
+        rewrite HexprD'_conv in H12. autorewrite_with_eq_rw_in H12.
+        rewrite HexprD'_conv in H13. autorewrite_with_eq_rw_in H13.
+        forwardy. inv_all. subst.
+
+        generalize (@vars_to_uvars_sound typ (expr typ func) _ _ _ _ _ _ _ _ nil _ _ _ H12).
+        simpl. destruct 1 as [ ? [ HexprD'e_subst ? ] ].
+        eapply exprD'_weakenV with (tvs':=getVars ctx) in HexprD'e_subst; eauto.
+        simpl in HexprD'e_subst. forward_reason.
+        assert (t = t0) by eauto using RD_single_type.
+        intros; subst.
+        replace (length (getUVars ctx ++ t0 :: nil))
+           with (S (length (getUVars ctx))) in H17
+             by (rewrite app_length; simpl; omega).
+        eapply exprD'_weakenU
+          with (tus':=l0.(vars)) in HexprD'e; eauto.
+        destruct (drop_exact_append_exact (vars l0) (getUVars ctx)) as [ ? [ Hx ? ] ].
+        rewrite Hx in *; clear Hx.
+        destruct (pctxD_substD H2 HpctxDcs) as [ ? [ Hx ? ] ].
+        rewrite Hx in *; clear Hx.
+        destruct HexprD'e as [ ? [ Hx ? ] ].
+        specialize (H6 _ _ _ H16 Hx eq_refl).
+        clear Hx.
+        forward_reason.
+        generalize (pctxD_SubstMorphism_progress H6).
+        simpl. rewrite HpctxDcs.
+        intro Hx; specialize (Hx _ eq_refl). destruct Hx.
+        rewrite H23 in *.
+        assert (exists Ps,
+                   goalD (getUVars ctx ++ vars l0) (getVars ctx)
+                         (GConj_list
+                            (map
+                               (fun e2 : expr typ func =>
+                                  GGoal (vars_to_uvars 0 (length (getUVars ctx)) e2))
+                               (premises l0))) = Some Ps /\
+                   forall (us : hlist typD (getUVars ctx)) us' vs,
+                     Ps (hlist_app us us') vs <->
+                     Forall (fun y => y us (hlist_app us' Hnil)) y).
+        { revert H0.
+          destruct l0. simpl in *.
+          clear - RTypeOk_typD RSymOk_func Typ2Ok_Fun.
+          intros.
+          cut (exists Ps : exprT (getUVars ctx ++ vars) (getVars ctx) Prop,
+                  goalD (getUVars ctx ++ vars) (getVars ctx)
+                        (GConj_list_simple
+                           (map
+                              (fun e2 : expr typ func =>
+                                 GGoal (vars_to_uvars 0 (length (getUVars ctx)) e2))
+                              premises)) = Some Ps /\
+                  (forall (us : hlist typD (getUVars ctx)) (us' : hlist typD vars)
+                          (vs : hlist typD (getVars ctx)),
+                      Ps (hlist_app us us') vs <->
+                      Forall
+                        (fun
+                            y0 : hlist typD (getUVars ctx) ->
+                                 hlist typD (vars ++ nil) -> Prop =>
+                            y0 us (hlist_app us' Hnil)) y)).
+          { destruct (goalD_GConj_list_GConj_list_simple
+                        (getUVars ctx ++ vars) (getVars ctx)
+                        (map (fun e2 : expr typ func =>
+                                GGoal (vars_to_uvars 0 (length (getUVars ctx)) e2))
+                           premises)).
+            { intros; forward_reason; congruence. }
+            { intros; forward_reason.
+              inv_all. subst. eexists; split; eauto.
+              intros.
+              rewrite <- H2. eapply H.
+              reflexivity. reflexivity. } }
+          revert H0. revert y.
+          induction premises; simpl; intros.
+          { eexists; split; eauto.
+            simpl. inv_all. subst.
+            split; eauto. }
+          { simpl in *.
+            forwardy. inv_all. subst.
+            unfold exprD'_typ0 in H.
+            simpl in H. forwardy.
+            generalize (@vars_to_uvars_sound typ (expr typ func) _ _ _ _ _ _ _ _ nil _ _ _ H).
+            intro. forward_reason.
+            unfold propD, exprD'_typ0.
+            simpl in H2.
+            eapply exprD'_weakenV
+              with (tvs':=getVars ctx)
+                in H2; eauto.
+            forward_reason. simpl in H2.
+            generalize (@exprD'_conv typ _ (expr typ func) _); eauto. simpl.
+            intro Hx.
+            rewrite Hx
+               with (pfu:=f_equal _ (eq_sym (app_nil_r_trans _))) (pfv:=eq_refl)
+                 in H2.
+            autorewrite_with_eq_rw_in H2.
+            forwardy.
+            rewrite H2.
+            specialize (IHpremises _ H0).
+            forward_reason. rewrite H6.
+            eexists; split; eauto. simpl.
+            intros.
+            inv_all. subst.
+            intros. rewrite Forall_cons_iff.
+            rewrite <- (H7 _ _ vs).
+            autorewrite with eq_rw.
+            specialize (H3 us (hlist_app us' Hnil) Hnil).
+            simpl in *.
+            rewrite H3; clear H3.
+            erewrite (H4 (hlist_app us (hlist_app us' Hnil)) Hnil vs); clear H4.
+            simpl. rewrite hlist_app_nil_r.
+            unfold f_equal.
+            autorewrite with eq_rw.
+            clear.
+            generalize (app_nil_r_trans vars).
+            generalize dependent (vars ++ nil).
+            intros; subst. reflexivity. } }
+        destruct H24 as [ ? [ Hx ? ] ].
+        rewrite Hx in *; clear Hx.
+        forwardy.
+        rewrite (ctx_subst_eta c0) in H7.
+        simpl in H7.
+        forwardy. rewrite H26.
+        inv_all; subst.
+        destruct (amap_substD_amap_empty (getUVars ctx ++ vars l0)
+                                         (getVars ctx)) as [ ? [ Hx ? ] ];
+          change_rewrite Hx in H6; clear Hx.
+        rewrite HpctxDcs in H6.
+        simpl in *.
+        destruct (drop_exact_append_exact l0.(vars) (getUVars ctx)) as [ ? [ Hx ? ] ];
+          rewrite Hx in *; clear Hx.
+        destruct H25.
+        inv_all. subst.
+        forwardy.
+        repeat match goal with
+               | H : ?X = _ , H' : ?X = _ |- _ => rewrite H in H'
+               end.
+        forward_reason; inv_all; subst.
+        simpl in *.
+        rewrite H7 in *.
+        rewrite H4 in *.
+        rewrite H6 in *.
+        rewrite H26 in *.
+        inv_all.
+        forwardy.
+        generalize H7. intro Hamap_substD.
+        eapply subst_getInstantiation in H7;
+          eauto using WellFormed_entry_WellFormed_pre_entry
+                 with typeclass_instances.
+        destruct H7.
+        assert (exists e'D,
+                   exprD' (getUVars ctx) (getVars ctx) t0
+                          (instantiate (fun u : ExprI.uvar => amap_lookup u x12)
+                                       0 (vars_to_uvars 0 (length (getUVars ctx)) l0.(concl).(rhs))) = Some e'D /\
+                   forall us vs,
+                     e'D us vs =
+                     y0 us (hlist_map
+                              (fun (t : typ) (x6 : exprT (getUVars ctx) (getVars ctx) (typD t)) =>
+                                 x6 us vs) x5)).
+        { (** this says that I can strengthen the expression **)
+          (** TODO: This should be a lemma **)
+          revert H13. revert H. revert H5. revert Hamap_substD.
+          clear - RTypeOk_typD RSymOk_func Typ2Ok_Fun H40.
+          generalize dependent (getVars ctx).
+          generalize dependent (rhs (concl l0)).
+          generalize dependent (vars l0).
+          clear - RType_typD RTypeOk_typD RSymOk_func Typ2Ok_Fun.
+          intros.
+          generalize (@vars_to_uvars_sound typ (expr typ func) _ _ _ _ _ _ _ e nil t0 l _ H13).
+          destruct 1 as [ ? [ ? ? ] ].
+          eapply ExprI.exprD'_weakenV with (tvs':=t) in H0; eauto with typeclass_instances.
+          destruct H0 as [ ? [ ? ? ] ].
+          destruct (@instantiate_sound typ (expr typ func) _ _ _ (getUVars ctx++l) t
+                                       (fun u : ExprI.uvar => amap_lookup u x12)
+                                       (vars_to_uvars 0 (length (getUVars ctx)) e) nil t0 x0 y3).
+          { generalize (@sem_preserves_if_substD (amap (expr typ func)) typ (expr typ func) RType_typD (Expr_expr _ _ _ _) _ _).
+            simpl. intro. eapply H3.
+            2: eapply Hamap_substD.
+            eapply WellFormed_entry_WellFormed_pre_entry in H40.
+            destruct H40. assumption. }
+          { eassumption. }
+          { destruct H3.
+            eapply exprD'_strengthenU_multi in H3.
+            2: eauto with typeclass_instances.
+            { destruct H3 as [ ? [ ? ? ] ].
+              eexists; split; try eassumption.
+              intros.
+              specialize (H us vs).
+              specialize (H4 _ _ Hnil H).
+              simpl in *.
+              symmetry.
+              etransitivity; [ eapply (H1 _ _ Hnil) | ].
+              etransitivity; [ eapply H2 | ].
+              etransitivity; [ eapply H4 | ].
+              eapply H6. }
+            { intros.
+              clear H2 H1 H3 H4 H.
+              match goal with
+              | |- ?X = _ => consider X; try reflexivity; intro
+              end.
+              exfalso.
+              eapply mentionsU_instantiate in H.
+              assert (amap_lookup (length (getUVars ctx) + u) x12 <> None).
+              { clear - H5 H40 H6.
+                destruct H40.
+                clear H0.
+                red in H.
+                destruct H as [ ? [ ? ? ] ].
+                clear H H1.
+                generalize dependent (length (getUVars ctx)).
+                generalize dependent (length l).
+                clear.
+                intros.
+                eapply pigeon_principle; eauto. }
+              destruct H.
+              { destruct H. eauto. }
+              { destruct H. destruct H. destruct H as [ ? [ ? ? ] ].
+                destruct H40.
+                consider (amap_lookup (length (getUVars ctx) + u) x12); intros; try congruence.
+                eapply FMapSubst.SUBST.normalized_fmapsubst in H1.
+                3: eapply H.
+                cut (true = false); [ clear; intros; congruence | ].
+                rewrite <- H3. rewrite <- H1. reflexivity.
+                destruct H4. assumption. } } } }
+        destruct H7 as [ ? [ Hx ? ] ]; rewrite Hx; clear Hx.
+        split.
+        { etransitivity; eassumption. }
+        intros.
+        eapply pctxD_substD' with (us:=us) (vs:=vs) in H37; eauto with typeclass_instances.
+        gather_facts.
+        eapply pctxD_SubstMorphism; [ | | eauto | ]; eauto.
+        gather_facts.
+        eapply pctxD_SubstMorphism; [ | | eauto | ]; eauto.
+        gather_facts.
+        eapply Pure_pctxD; eauto. intros.
+        specialize (H us0 vs0).
+        specialize (H7 us0 vs0).
+        generalize dependent (hlist_map
+           (fun (t : typ) (x6 : exprT (getUVars ctx) (getVars ctx) (typD t)) =>
+            x6 us0 vs0) x5); simpl; intros.
+        apply (H10 _ us0 _) in H9; clear H10.
+        rewrite foralls_sem in H9.
+        setoid_rewrite impls_sem in H9.
+        generalize (H9 h); clear H9.
+        rewrite Quant._forall_sem in H25.
+        simpl.
+        specialize (H25 _ H).
+        specialize (H23 _ H).
+        specialize (H21 _ H23).
+        rewrite H7; clear H7.
+        rewrite (H20 us0 vs0 h); clear H20.
+        specialize (H22 (hlist_app us0 h) vs0).
+        rewrite H28 in H22.
+        specialize (H22 (conj H23 H19)).
+        forward_reason.
+        specialize (H9 Hnil).
+        simpl in H9.
+        rewrite <- H9; clear H9.
+        specialize (fun X => H17 X Hnil); simpl in H17.
+        rewrite <- H17; clear H17.
+        rewrite <- H15; clear H15.
+        rewrite hlist_app_nil_r.
+        autorewrite with eq_rw.
+        simpl.
+        refine (fun x => x _).
+        clear x14.
+        eapply List.Forall_map.
+        eapply H24 in H25.
+        revert H25.
+        eapply Forall_impl.
+        intro. rewrite hlist_app_nil_r. tauto. }
+      { exfalso; clear - H3; inversion H3. }
+    Time Qed.
+  End core_rewrite.
+
+  (* This section implements the re-indexing operation
+   * to run [rtac]'s from [mrw]. Note that the main thing to do
+   * is extend the context with any extra variables and re-index
+   * variables in the term.
+   *)
+  Section reindexing.
+    (* This has to do with converting expressions for tactics *)
+    Let _lookupU (u : ExprI.uvar) : option (expr typ func) := None.
+    Let _lookupV (under : nat) (above : nat) (v : ExprI.var)
+    : option (expr typ func) :=
+      Some (Var (if v ?[ ge ] under
+                 then v - under
+                 else v + above)).
+
+    Definition expr_convert (u : nat) (above : nat)
+    : expr typ func -> expr typ func :=
+      expr_subst _lookupU (_lookupV u above) 0.
+
+    (** TODO(gmalecha): Move to EnvI or ExtLib.Data.HList **)
+    Lemma nth_error_get_hlist_nth_appR'
+    : forall T (F : T -> Type) ls u v,
+        nth_error_get_hlist_nth F ls u = Some v ->
+        forall ls',
+        exists v',
+          nth_error_get_hlist_nth F (ls' ++ ls) (u + length ls') = Some (existT _ (projT1 v) v') /\
+          forall a b,
+            projT2 v a = v' (hlist_app b a).
+    Proof using.
+      induction ls'.
+      { simpl.
+        replace (u + 0) with u by omega.
+        destruct v. eexists; split; eauto.
+        simpl. intros.
+        rewrite (hlist_eta b). reflexivity. }
+      { simpl.
+        replace (u + S (length ls')) with (S (u + length ls')) by omega.
+        destruct IHls' as [ ? [ ? ? ] ].
+        rewrite H0. eexists; split; eauto.
+        simpl. intros.
+        rewrite (hlist_eta b). simpl. eauto. }
+    Qed.
+
+    Lemma expr_convert_sound
+    : forall tus tvs tvs' e t eD,
+        exprD' tus (tvs ++ tvs') t e = Some eD ->
+        exists eD',
+          exprD' tus (tvs' ++ tvs) t (expr_convert (length tvs) (length tvs') e) = Some eD' /\
+          forall a b c,
+            eD a (hlist_app b c) = eD' a (hlist_app c b).
+    Proof.
+      clear - Typ2Ok_Fun RTypeOk_typD RSymOk_func.
+      unfold expr_convert.
+      intros.
+      destruct (fun Hu Hv => @ExprI.expr_subst_sound
+                    typ _ (expr typ func) (Expr_expr _ _ _ _) _
+                    _lookupU
+                    (_lookupV (length tvs) (length tvs'))
+                    0 e _ eq_refl nil
+                    tus (tvs ++ tvs') tus (tvs' ++ tvs)
+                    (fun us vs us' vs' =>
+                       us = us' /\
+                       let (_vs,_vs') := hlist_split _ _ vs in
+                       let (__vs,__vs') := hlist_split _ _ vs' in
+                       _vs = __vs' /\ _vs' = __vs) Hu Hv t _ eq_refl H).
+      { simpl. clear.
+        intros. eexists; split; eauto.
+        intros. destruct H1; subst; auto. }
+      { simpl. intros.
+        autorewrite with exprD_rw. simpl.
+        consider (u ?[ ge ] length tvs); intros.
+        { eapply nth_error_get_hlist_nth_appR in H1; eauto.
+          simpl in H1. forward_reason.
+          eapply nth_error_get_hlist_nth_weaken with (ls':=tvs) in H1.
+          simpl in H1.
+          forward_reason. rewrite H1.
+          rewrite type_cast_refl; eauto.
+          eexists; split; eauto.
+          unfold Rcast_val, Rcast, Relim. simpl.
+          intros.
+          revert H5.
+          rewrite <- (hlist_app_hlist_split _ _ vs).
+          rewrite <- (hlist_app_hlist_split _ _ vs').
+          rewrite hlist_split_hlist_app.
+          rewrite hlist_split_hlist_app.
+          destruct 1.
+          rewrite H3. rewrite <- H4.
+          f_equal. tauto. }
+        { assert (u < length tvs) by omega.
+          eapply nth_error_get_hlist_nth_appL in H3.
+          destruct H3. destruct H3.
+          rewrite H3 in H1.
+          assert (u + length tvs' >= length tvs') by omega.
+          destruct H4 as [ ? [ ? ? ] ].
+          eapply nth_error_get_hlist_nth_appR' in H4; simpl in H4.
+          destruct H4 as [ ? [ ? ? ] ].
+          rewrite H4.
+          inv_all. subst. simpl.
+          rewrite type_cast_refl; eauto.
+          eexists; split; eauto.
+          intros us vs us' vs'.
+          rewrite <- (hlist_app_hlist_split _ _ vs).
+          rewrite <- (hlist_app_hlist_split _ _ vs').
+          rewrite hlist_split_hlist_app.
+          rewrite hlist_split_hlist_app.
+          destruct 1.
+          simpl in *.
+          rewrite H6. rewrite <- H7.
+          unfold Rcast_val, Rcast; simpl. f_equal. tauto. } }
+      { simpl in H0.
+        destruct H0; eexists; split; eauto.
+        intros. apply (H1 a (hlist_app b c) a (hlist_app c b) Hnil).
+        split; auto.
+        do 2 rewrite hlist_split_hlist_app.
+        tauto. }
+    Qed.
+
+    (* This code starts to build the structure necessary for [rtac]
+     *)
+    Fixpoint wrap_tvs (tvs : tenv typ) (ctx : Ctx typ (expr typ func))
+    : Ctx typ (expr typ func) :=
+      match tvs with
+      | nil => ctx
+      | t :: tvs' => wrap_tvs tvs' (CAll ctx t)
+      end.
+
+    Fixpoint wrap_tvs_ctx_subst tvs ctx (cs : ctx_subst ctx)
+    : ctx_subst (wrap_tvs tvs ctx) :=
+      match tvs as tvs return ctx_subst (wrap_tvs tvs ctx) with
+      | nil => cs
+      | t :: tvs => wrap_tvs_ctx_subst _ (AllSubst cs)
+      end.
+
+    Fixpoint unwrap_tvs_ctx_subst T tvs ctx
+    : ctx_subst (wrap_tvs tvs ctx) -> (ctx_subst ctx -> T) -> T :=
+      match tvs as tvs
+            return ctx_subst (wrap_tvs tvs ctx) -> (ctx_subst ctx -> T) -> T
+      with
+      | nil => fun cs k => k cs
+      | t :: tvs => fun cs k =>
+        @unwrap_tvs_ctx_subst T tvs (CAll ctx t) cs (fun z => k (fromAll z))
+      end.
+
+    (* TODO(gmalecha): This does not have a stand-alone soundness theorem,
+     * which is problematic because it does some quite complex manipulation.
+     *)
+    Definition for_tactic
+               (m : expr typ func ->
+                    tenv typ -> tenv typ -> nat -> nat ->
+                    forall ctx : Ctx typ (expr typ func),
+                      ctx_subst ctx -> option (expr typ func * ctx_subst ctx))
+    : expr typ func -> mrw (expr typ func) :=
+      fun e tvs' tus tvs nus nvs ctx cs =>
+        let under := length tvs' in
+        let e' := expr_convert under nvs e in
+        match
+          m e' tus (tvs ++ tvs') nus (under + nvs) _
+            (@wrap_tvs_ctx_subst tvs' ctx cs)
+        with
+        | None => None
+        | Some (v,cs') =>
+          Some (expr_convert nvs under v,
+                @unwrap_tvs_ctx_subst _ tvs' ctx cs' (fun x => x))
+        end.
+
+    (* TODO(gmalecha): This should go in a new file that implements
+     * rewriting databases.
+     *)
+    Fixpoint using_rewrite_db'
+             (ls : list (rw_lemma typ func Rbase * rtacK typ (expr typ func)))
+    : expr typ func -> R ->
+      tenv typ -> tenv typ -> nat -> nat ->
+      forall ctx, ctx_subst ctx -> option (expr typ func * ctx_subst ctx) :=
+      match ls with
+      | nil => fun _ _ _ _ _ _ _ _ => None
+      | (lem,tac) :: ls =>
+        let res := using_rewrite_db' ls in
+        let crw := core_rewrite lem tac in
+        fun e r tus tvs nus nvs ctx cs =>
+          if Req_dec Rbase_eq r lem.(concl).(rel) then
+            match crw e tus tvs nus nvs ctx cs with
+            | None => res e r tus tvs nus nvs ctx cs
+            | X => X
+            end
+          else res e r tus tvs nus nvs ctx cs
+      end.
+
+    Definition using_rewrite_db
+               (ls : list (rw_lemma typ func Rbase * rtacK typ (expr typ func)))
+    : expr typ func -> R -> mrw (expr typ func) :=
+      let rw_db := using_rewrite_db' ls in
+      fun e r => for_tactic (fun e => rw_db e r) e.
+
+    Definition using_prewrite_db
+        (lems : expr typ func -> list (rw_lemma typ func Rbase * rtacK typ (expr typ func)))
+    : expr typ func -> R -> mrw (expr typ func) :=
+      fun e r =>
+        for_tactic (fun e => using_rewrite_db' (lems e) e r) e.
+
+    Lemma using_rewrite_db'_sound
+    : forall r ctx (cs : ctx_subst ctx),
+        let tus := getUVars ctx in
+        let tvs := getVars ctx in
+        forall hints : list (rw_lemma typ func Rbase * rtacK typ (expr typ func)),
+        Forall (fun lt =>
+                  lemmaD (rw_conclD RbaseD) nil nil (fst lt) /\
+                  rtacK_sound (snd lt)) hints ->
+        forall e e' cs',
+          @using_rewrite_db' hints e r tus tvs (length tus) (length tvs) ctx cs = Some (e', cs') ->
+          WellFormed_ctx_subst cs ->
+          WellFormed_ctx_subst cs' /\
+          (forall (t : typ) (rD : typD t -> typD t -> Prop),
+              RD RbaseD r t = Some rD ->
+              match pctxD cs with
+              | Some _ =>
+                match exprD' tus tvs t e with
+                | Some eD =>
+                  match pctxD cs' with
+                  | Some csD' =>
+                    match exprD' tus tvs t e' with
+                    | Some eD' =>
+                      SubstMorphism cs cs' /\
+                      (forall (us : hlist typD (getAmbientUVars ctx))
+                              (vs : hlist typD (getAmbientVars ctx)),
+                          csD'
+                            (fun (us0 : hlist typD (getUVars ctx))
+                                 (vs0 : hlist typD (getVars ctx)) =>
+                                 rD (eD us0 vs0)
+                                    (eD' us0 vs0)) us vs)
+                    | None => False
+                    end
+                  | None => False
+                  end
+                | None => True
+                end
+              | None => True
+              end).
+    Proof.
+      induction 1.
+      { simpl. inversion 1. }
+      { simpl. intros. destruct x.
+        assert (using_rewrite_db' l e r tus tvs (length tus) (length tvs) cs = Some (e',cs')
+             \/ (r = l0.(concl).(rel) /\
+                 core_rewrite l0 r0 e tus tvs (length tus) (length tvs) cs = Some (e',cs'))).
+        { generalize (Req_dec_ok Rbase_eq Rbase_eq_ok r l0.(concl).(rel)).
+          destruct (Req_dec Rbase_eq r l0.(concl).(rel)); eauto.
+          intros. destruct (core_rewrite l0 r0 e tus tvs (length tus) (length tvs) cs); eauto. }
+        clear H1. destruct H3; eauto.
+        destruct H1. subst. clear IHForall H0.
+        simpl in H. destruct H.
+        revert H2. revert H3. revert H. revert H0.
+        intros.
+        eapply core_rewrite_sound in H3; eauto. }
+    Qed.
+
+    Lemma getAmbientUVars_wrap_tvs : forall tvs ctx,
+        getAmbientUVars (wrap_tvs tvs ctx) = getAmbientUVars ctx.
+    Proof using.
+      induction tvs; simpl. reflexivity.
+      intros. rewrite IHtvs. reflexivity.
+    Defined.
+
+    Lemma getAmbientVars_wrap_tvs : forall tvs ctx,
+        getAmbientVars (wrap_tvs tvs ctx) = getAmbientVars ctx.
+    Proof using.
+      induction tvs; simpl. reflexivity.
+      intros. rewrite IHtvs. reflexivity.
+    Defined.
+
+    Lemma getVars_wrap_tvs : forall tvs' ctx,
+        getVars (wrap_tvs tvs' ctx) = getVars ctx ++ tvs'.
+    Proof using.
+      induction tvs'; simpl; eauto.
+      symmetry. eapply app_nil_r_trans.
+      simpl. intros. rewrite IHtvs'. simpl.
+      rewrite app_ass_trans. reflexivity.
+    Defined.
+
+    Lemma WellFormed_ctx_subst_unwrap_tvs
+    : forall tvs' ctx ctx' (cs : ctx_subst _)
+             (k : ctx_subst (Ctx_append ctx ctx') -> ctx_subst ctx),
+        (forall cs, WellFormed_ctx_subst cs -> WellFormed_ctx_subst (k cs)) ->
+        WellFormed_ctx_subst cs ->
+        WellFormed_ctx_subst
+          (@unwrap_tvs_ctx_subst (ctx_subst ctx) tvs' (Ctx_append ctx ctx') cs k).
+    Proof using.
+      induction tvs'; simpl; auto.
+      intros. specialize (IHtvs' ctx (CAll ctx' a) cs).
+      simpl in *. eapply IHtvs'; eauto.
+      intros. eapply H. rewrite (ctx_subst_eta cs0) in H1.
+      inv_all. assumption.
+    Qed.
+
+    Fixpoint unwrap_tvs_ctx_subst' (tvs : tenv typ) (ctx : Ctx typ (expr typ func))
+    : ctx_subst (wrap_tvs tvs ctx) -> ctx_subst ctx :=
+      match tvs as tvs return ctx_subst (wrap_tvs tvs ctx) -> ctx_subst ctx with
+      | nil => fun X => X
+      | t :: tvs => fun X => fromAll (unwrap_tvs_ctx_subst' tvs _ X)
+      end.
+
+    Theorem unwrap_tvs_ctx_subst_unwrap_tvs_ctx_subst'
+    : forall T tvs ctx cs (k : _ -> T),
+        k (@unwrap_tvs_ctx_subst' tvs ctx cs) =
+        unwrap_tvs_ctx_subst tvs cs k.
+    Proof using.
+      induction tvs; simpl. auto.
+      intros. rewrite <- IHtvs. reflexivity.
+    Qed.
+
+    (** TODO: Move **)
+    Lemma pctxD_iff : forall ctx (cs : ctx_subst ctx) cD P Q,
+        pctxD cs = Some cD ->
+        (forall us vs, P us vs <-> Q us vs) ->
+        forall us vs,
+          cD P us vs <-> cD Q us vs.
+    Proof using.
+      intros.
+      split; eapply Ap_pctxD; eauto; eapply Pure_pctxD; eauto; intros; eapply H0; eauto.
+    Qed.
+
+    (** TODO: Move **)
+    Lemma forall_hlist_nil : forall T (F : T -> Type) (P : hlist F nil -> Prop),
+        (forall x, P x) <-> P Hnil.
+    Proof using.
+      intros. split. eauto. intros. rewrite hlist_eta. assumption.
+    Qed.
+
+    Lemma forall_hlist_cons : forall T (F : T -> Type) t ts (P : hlist F (t :: ts) -> Prop),
+        (forall x, P x) <-> (forall x xs, P (Hcons x xs)).
+    Proof.
+      intros. split. eauto. intros. rewrite hlist_eta. eapply H.
+    Qed.
+
+    Lemma getUVars_wrap_tvs
+    : forall tvs' ctx, getUVars (wrap_tvs tvs' ctx) = getUVars ctx.
+    Proof using.
+      induction tvs'; simpl; auto.
+      intros.  rewrite IHtvs'. reflexivity.
+    Defined.
+
+    Lemma WellFormed_ctx_subst_wrap_tvs : forall tvs' ctx (cs : ctx_subst ctx),
+        WellFormed_ctx_subst cs ->
+        WellFormed_ctx_subst (wrap_tvs_ctx_subst tvs' cs).
+    Proof using.
+      induction tvs'; simpl; auto.
+      intros. eapply IHtvs'. constructor. assumption.
+    Qed.
+
+    Lemma pctxD_unwrap_tvs_ctx_subst
+    : forall tvs ctx (cs : ctx_subst _) cD,
+        pctxD cs = Some cD ->
+        exists cD',
+          pctxD (@unwrap_tvs_ctx_subst _ tvs ctx cs (fun x => x)) = Some cD' /\
+          forall (us : hlist typD _) (vs : hlist typD _) (P : exprT _ _ Prop),
+            cD' (fun us vs => forall vs', P us (hlist_app vs vs')) us vs <->
+            cD match eq_sym (getVars_wrap_tvs tvs ctx) in _ = V
+                   , eq_sym (getUVars_wrap_tvs tvs ctx) in _ = U
+                     return exprT U V Prop
+               with
+               | eq_refl , eq_refl => P
+               end
+               match eq_sym (getAmbientUVars_wrap_tvs tvs ctx) in _ = V
+                     return hlist _ V
+               with
+               | eq_refl => us
+               end
+               match eq_sym (getAmbientVars_wrap_tvs tvs ctx) in _ = V
+                     return hlist _ V
+               with
+               | eq_refl => vs
+               end.
+    Proof.
+      clear - RTypeOk_typD RSymOk_func Typ2Ok_Fun.
+      intros. rewrite <- unwrap_tvs_ctx_subst_unwrap_tvs_ctx_subst'.
+      generalize dependent cD. revert cs. revert ctx.
+      induction tvs.
+      { simpl. eauto.
+        eexists; split; eauto.
+        intros.
+        eapply pctxD_iff; eauto.
+        intros.
+        rewrite forall_hlist_nil.
+        rewrite hlist_app_nil_r.
+        generalize (app_nil_r_trans (getVars ctx)).
+        clear. generalize dependent (getVars ctx ++ nil).
+        intros; subst. reflexivity. }
+      { simpl; intros.
+        specialize (@IHtvs _ _ _ H).
+        forward_reason.
+        generalize dependent (unwrap_tvs_ctx_subst' tvs (CAll ctx a) cs).
+        intro. rewrite (ctx_subst_eta c); simpl.
+        intros; forwardy.
+        eexists; split; eauto.
+        inv_all. subst. intros.
+        specialize (H1 us vs
+                       match eq_sym (app_ass_trans (getVars ctx) (a::nil) _) in _ = X
+                             return exprT _ X Prop
+                       with
+                       | eq_refl => P
+                       end).
+        simpl in *.
+        etransitivity; [ etransitivity; [ | eapply H1 ] | ]; clear H1.
+        { eapply pctxD_iff; eauto.
+          intros.
+          rewrite forall_hlist_cons.
+          eapply Data.Prop.forall_iff; intros.
+          eapply Data.Prop.forall_iff; intros.
+          rewrite hlist_app_assoc.
+          clear. simpl.
+          generalize dependent (app_ass_trans (getVars ctx) (a :: nil) tvs).
+          simpl in *.
+          generalize dependent ((getVars ctx ++ a :: nil) ++ tvs).
+          intros; subst. reflexivity. }
+        { clear - H.
+          match goal with
+          | |- _ _ ?U ?V <-> _ _ ?U' ?V' =>
+            replace V with V' ; [ replace U with U' | ]
+          end.
+          { eapply pctxD_iff; eauto; clear.
+            generalize (app_ass_trans (getVars ctx) (a :: nil) tvs).
+            generalize (getVars_wrap_tvs tvs (CAll ctx a)).
+            generalize (getUVars_wrap_tvs tvs (CAll ctx a)).
+            simpl.
+            intros;
+            repeat match goal with
+               | H : @eq (tenv typ) ?X ?Y |- _ =>
+                 first [ generalize dependent X | generalize dependent Y ] ; intros; subst
+               | H : @eq (list typ) ?X ?Y |- _ =>
+                 first [ generalize dependent X | generalize dependent Y ] ; intros; subst
+               end. reflexivity. }
+          { clear.
+            generalize (getAmbientUVars_wrap_tvs tvs (CAll ctx a)).
+            simpl in *. destruct e. reflexivity. }
+          { clear.
+            generalize (getAmbientVars_wrap_tvs tvs (CAll ctx a)).
+            simpl. destruct e. reflexivity. } } }
+    Qed.
+
+    Lemma pctxD_wrap_tvs_ctx_subst
+    : forall tvs ctx (cs : ctx_subst ctx) cD,
+        pctxD cs = Some cD ->
+        exists cD',
+          pctxD (wrap_tvs_ctx_subst tvs cs) = Some cD' /\
+          forall us vs (P : exprT _ _ Prop),
+            cD (fun us vs => forall vs', P us (hlist_app vs vs')) us vs <->
+            cD' match eq_sym (getVars_wrap_tvs tvs ctx) in _ = V
+                                                           , eq_sym (getUVars_wrap_tvs tvs ctx) in _ = U
+                      return exprT U V Prop
+                with
+                | eq_refl , eq_refl => P
+                end
+                match eq_sym (getAmbientUVars_wrap_tvs tvs ctx) in _ = V
+                      return hlist _ V
+                with
+                | eq_refl => us
+                end
+                match eq_sym (getAmbientVars_wrap_tvs tvs ctx) in _ = V
+                      return hlist _ V
+                with
+                | eq_refl => vs
+                end.
+    Proof using RTypeOk_typD RSymOk_func Typ2Ok_Fun.
+      induction tvs.
+      { simpl. eauto.
+        eexists; split; eauto.
+        intros; eapply pctxD_iff; eauto.
+        intros. rewrite forall_hlist_nil.
+        rewrite hlist_app_nil_r. clear.
+        generalize (app_nil_r_trans (getVars ctx)).
+        generalize dependent (getVars ctx ++ nil). intros; subst.
+        reflexivity. }
+      { simpl. intros.
+        specialize (IHtvs (CAll ctx a) (AllSubst cs)).
+        simpl in IHtvs. rewrite H in IHtvs.
+        specialize (IHtvs _ eq_refl).
+        destruct IHtvs as [ ? [ ? ? ] ].
+        eexists; split; eauto.
+        intros.
+        specialize (H1 us vs
+                       match eq_sym (app_ass_trans (getVars ctx) (a::nil) _) in _ = X
+                             return exprT _ X Prop
+                       with
+                       | eq_refl => P
+                       end).
+        etransitivity; [ etransitivity; [ | eapply H1 ] | ]; clear H1.
+        { eapply pctxD_iff; eauto.
+          intros. rewrite forall_hlist_cons.
+          eapply Data.Prop.forall_iff; intro.
+          eapply Data.Prop.forall_iff; intro.
+          rewrite hlist_app_assoc.
+          clear.
+          generalize dependent (eq_sym (app_ass_trans (getVars ctx) (a :: nil) tvs)).
+          simpl in *. destruct e. reflexivity. }
+        { match goal with
+          | |- _ _ ?U ?V <-> _ _ ?U' ?V' =>
+            replace V with V' ; [ replace U with U' | ]
+          end.
+          { eapply pctxD_iff; eauto.
+            intros.
+            generalize (app_ass_trans (getVars ctx) (a :: nil) tvs).
+            generalize (getVars_wrap_tvs tvs (CAll ctx a)).
+            generalize (getUVars_wrap_tvs tvs (CAll ctx a)).
+            simpl. clear.
+            intros;
+            repeat match goal with
+               | H : @eq (tenv typ) ?X ?Y |- _ =>
+                 first [ generalize dependent X | generalize dependent Y ] ; intros; subst
+               | H : @eq (list typ) ?X ?Y |- _ =>
+                 first [ generalize dependent X | generalize dependent Y ] ; intros; subst
+               end. reflexivity. }
+          { clear.
+            generalize (getAmbientUVars_wrap_tvs tvs (CAll ctx a)).
+            simpl in *. destruct e. reflexivity. }
+          { clear.
+            generalize (getAmbientVars_wrap_tvs tvs (CAll ctx a)).
+            simpl. destruct e. reflexivity. } } }
+    Qed.
+
+    Lemma SubstMorphism_wrap_tvs_ctx_subst
+    : forall tvs' ctx cs c,
+        SubstMorphism (wrap_tvs_ctx_subst tvs' cs) c ->
+        SubstMorphism cs
+                      (unwrap_tvs_ctx_subst tvs' c (fun x : ctx_subst ctx => x)).
+    Proof.
+      clear. intros.
+      rewrite <- unwrap_tvs_ctx_subst_unwrap_tvs_ctx_subst'.
+      revert H. revert ctx c cs.
+      induction tvs'.
+      { simpl. tauto. }
+      { simpl. intros.
+        eapply IHtvs' in H.
+        inv_all. rewrite H. assumption. }
+    Qed.
+
+    Theorem using_rewrite_db_sound
+    : forall hints : list (rw_lemma typ func Rbase * rtacK typ (expr typ func)),
+        Forall (fun lt =>
+                  lemmaD (rw_conclD RbaseD) nil nil (fst lt) /\
+                  rtacK_sound (snd lt)) hints ->
+        setoid_rewrite_spec (fun e r =>
+                               rw_bind (using_rewrite_db hints e r)
+                                       (fun e => rw_ret (Progress e))).
+    Proof.
+      unfold using_rewrite_db.
+      unfold for_tactic.
+      red. red. intros.
+      unfold rw_bind in H0.
+      forwardy. inv_all. subst.
+      rewrite Plus.plus_comm in H0. rewrite <- app_length in H0.
+      destruct (fun Hx =>
+                    @using_rewrite_db'_sound r _ (wrap_tvs_ctx_subst tvs' cs) hints H
+                                             (expr_convert (length tvs') (length (getVars ctx)) e) e1 c0 Hx
+                                             (WellFormed_ctx_subst_wrap_tvs _ H1)).
+      { rewrite <- H0. f_equal.
+        eauto using getUVars_wrap_tvs.
+        eauto using getVars_wrap_tvs.
+        rewrite getUVars_wrap_tvs. reflexivity.
+        rewrite getVars_wrap_tvs. reflexivity. }
+      clear H0. subst.
+      split.
+      { eapply WellFormed_ctx_subst_unwrap_tvs
+          with (ctx':=CTop nil nil); eauto. }
+      intros.
+      specialize (H3 _ _ H0); clear H0.
+      destruct (pctxD cs) eqn:HpctxD_cs; trivial.
+      destruct (@pctxD_wrap_tvs_ctx_subst tvs' _ _ _ HpctxD_cs) as [ ? [ ? ? ] ].
+      rewrite H0 in H3.
+      destruct (exprD' (getUVars ctx) (tvs' ++ getVars ctx) t e) eqn:HexprD'_e; trivial.
+      generalize (@exprD'_conv typ _ (expr typ func) _). simpl.
+      intro Hconv.
+      rewrite Hconv
+         with (tus':=getUVars ctx) (tvs':=getVars ctx++tvs')
+              (pfu:=eq_sym (getUVars_wrap_tvs tvs' ctx)) (pfv:=eq_sym (getVars_wrap_tvs tvs' ctx))
+           in H3.
+      clear Hconv.
+      eapply expr_convert_sound in HexprD'_e.
+      destruct HexprD'_e as [ ? [ Hx ? ] ].
+      rewrite Hx in *; clear Hx.
+      autorewrite_with_eq_rw_in H3.
+      forwardy.
+      destruct (pctxD_unwrap_tvs_ctx_subst _ _ _ H3) as [ ? [ HpctxD_x1 ? ] ].
+      rewrite HpctxD_x1.
+      generalize (@exprD'_conv typ _ (expr typ func) _). simpl.
+      intro Hconv.
+      rewrite Hconv
+         with (pfu:=eq_sym (getUVars_wrap_tvs tvs' ctx)) (pfv:=eq_sym(getVars_wrap_tvs tvs' ctx))
+           in H6.
+      clear Hconv.
+      autorewrite_with_eq_rw_in H6.
+      forwardy; inv_all; subst.
+      eapply expr_convert_sound in H6.
+      destruct H6 as [ ? [ Hx ? ] ]; rewrite Hx; clear Hx.
+      destruct H7.
+      split.
+      { clear H9 H8 H4.
+        eapply SubstMorphism_wrap_tvs_ctx_subst; eauto. }
+      { intros.
+        specialize (H9 match
+                        eq_sym (getAmbientUVars_wrap_tvs tvs' ctx) in (_ = V)
+                        return (hlist typD V)
+                      with
+                      | eq_refl => us
+                      end
+                       match
+                         eq_sym (getAmbientVars_wrap_tvs tvs' ctx) in (_ = V)
+                         return (hlist typD V)
+                       with
+                       | eq_refl => vs
+                       end).
+        specialize (H8 us vs
+                   (fun us0 vs0 =>
+                      rD (x0 us0 vs0) (y2 us0 vs0))).
+        simpl in H8.
+        generalize dependent (getVars_wrap_tvs tvs' ctx).
+        generalize dependent (getUVars_wrap_tvs tvs' ctx).
+        generalize dependent (getAmbientUVars_wrap_tvs tvs' ctx).
+        generalize dependent (getAmbientVars_wrap_tvs tvs' ctx).
+        generalize (Ap_pctxD _ HpctxD_x1).
+        generalize (Pure_pctxD _ HpctxD_x1).
+        revert H5 H6 H7. clear.
+        generalize dependent (getAmbientVars (wrap_tvs tvs' ctx)).
+        generalize dependent (getAmbientUVars (wrap_tvs tvs' ctx)).
+        generalize dependent (getUVars (wrap_tvs tvs' ctx)).
+        generalize dependent (getVars (wrap_tvs tvs' ctx)).
+        intros; subst; simpl in *.
+        eapply H8 in H9; clear H8.
+        revert H9. eapply H0; clear H0.
+        eapply H; clear H.
+        clear - H5 H6.
+        intros. rewrite H5. rewrite <- H6. eauto. }
+    Time Qed.
+
+    (** TODO(gmalecha): This is almost identical to the above theorem *)
+    Theorem using_prewrite_db_sound
+    : forall hints : expr typ func ->
+                     list (rw_lemma typ func Rbase * rtacK typ (expr typ func)),
+        (forall e, Forall (fun lt =>
+                             lemmaD (rw_conclD RbaseD) nil nil (fst lt) /\
+                             rtacK_sound (snd lt)) (hints e)) ->
+        setoid_rewrite_spec (fun e r =>
+                               rw_bind (using_prewrite_db hints e r)
+                                       (fun e => rw_ret (Progress e))).
+    Proof.
+      intros.
+      unfold using_prewrite_db.
+      unfold for_tactic.
+      red. red. intros.
+      unfold rw_bind in H0.
+      forwardy. inv_all. subst.
+      rewrite Plus.plus_comm in H0. rewrite <- app_length in H0.
+      destruct (fun Hx =>
+                    @using_rewrite_db'_sound r _ (wrap_tvs_ctx_subst tvs' cs)
+                                             (hints (expr_convert (length tvs') (length (getVars ctx)) e)) (H _)
+                                             (expr_convert (length tvs') (length (getVars ctx)) e) e1 c0 Hx
+                                             (WellFormed_ctx_subst_wrap_tvs _ H1)).
+      { rewrite <- H0. f_equal.
+        eauto using getUVars_wrap_tvs.
+        eauto using getVars_wrap_tvs.
+        rewrite getUVars_wrap_tvs. reflexivity.
+        rewrite getVars_wrap_tvs. reflexivity. }
+      clear H0. subst.
+      split.
+      { eapply WellFormed_ctx_subst_unwrap_tvs
+          with (ctx':=CTop nil nil); eauto. }
+      intros.
+      specialize (H3 _ _ H0); clear H0.
+      destruct (pctxD cs) eqn:HpctxD_cs; trivial.
+      destruct (@pctxD_wrap_tvs_ctx_subst tvs' _ _ _ HpctxD_cs) as [ ? [ ? ? ] ].
+      rewrite H0 in H3.
+      destruct (exprD' (getUVars ctx) (tvs' ++ getVars ctx) t e) eqn:HexprD'_e; trivial.
+      generalize (@exprD'_conv typ _ (expr typ func) _). simpl.
+      intro Hconv.
+      rewrite Hconv
+         with (tus':=getUVars ctx) (tvs':=getVars ctx++tvs')
+              (pfu:=eq_sym (getUVars_wrap_tvs tvs' ctx)) (pfv:=eq_sym (getVars_wrap_tvs tvs' ctx))
+           in H3.
+      clear Hconv.
+      eapply expr_convert_sound in HexprD'_e.
+      destruct HexprD'_e as [ ? [ Hx ? ] ].
+      rewrite Hx in *; clear Hx.
+      autorewrite_with_eq_rw_in H3.
+      forwardy.
+      destruct (pctxD_unwrap_tvs_ctx_subst _ _ _ H3) as [ ? [ HpctxD_x1 ? ] ].
+      rewrite HpctxD_x1.
+      generalize (@exprD'_conv typ _ (expr typ func) _). simpl.
+      intro Hconv.
+      rewrite Hconv
+         with (pfu:=eq_sym (getUVars_wrap_tvs tvs' ctx)) (pfv:=eq_sym(getVars_wrap_tvs tvs' ctx))
+           in H6.
+      clear Hconv.
+      autorewrite_with_eq_rw_in H6.
+      forwardy; inv_all; subst.
+      eapply expr_convert_sound in H6.
+      destruct H6 as [ ? [ Hx ? ] ]; rewrite Hx; clear Hx.
+      destruct H7.
+      split.
+      { clear H9 H8 H4.
+        eapply SubstMorphism_wrap_tvs_ctx_subst; eauto. }
+      { intros.
+        specialize (H9 match
+                        eq_sym (getAmbientUVars_wrap_tvs tvs' ctx) in (_ = V)
+                        return (hlist typD V)
+                      with
+                      | eq_refl => us
+                      end
+                       match
+                         eq_sym (getAmbientVars_wrap_tvs tvs' ctx) in (_ = V)
+                         return (hlist typD V)
+                       with
+                       | eq_refl => vs
+                       end).
+        specialize (H8 us vs
+                   (fun us0 vs0 =>
+                      rD (x0 us0 vs0) (y2 us0 vs0))).
+        simpl in H8.
+        generalize dependent (getVars_wrap_tvs tvs' ctx).
+        generalize dependent (getUVars_wrap_tvs tvs' ctx).
+        generalize dependent (getAmbientUVars_wrap_tvs tvs' ctx).
+        generalize dependent (getAmbientVars_wrap_tvs tvs' ctx).
+        generalize (Ap_pctxD _ HpctxD_x1).
+        generalize (Pure_pctxD _ HpctxD_x1).
+        revert H5 H6 H7. clear.
+        generalize dependent (getAmbientVars (wrap_tvs tvs' ctx)).
+        generalize dependent (getAmbientUVars (wrap_tvs tvs' ctx)).
+        generalize dependent (getUVars (wrap_tvs tvs' ctx)).
+        generalize dependent (getVars (wrap_tvs tvs' ctx)).
+        intros; subst; simpl in *.
+        eapply H8 in H9; clear H8.
+        revert H9. eapply H0; clear H0.
+        eapply H; clear H.
+        clear - H5 H6.
+        intros. rewrite H5. rewrite <- H6. eauto. }
+    Qed.
+
+  End reindexing.
+
+  Section get_respectful.
+    (* This is just a "special" version of the rewriting lemma *)
+    Record Proper_concl : Type :=
+    { relation : R
+    ; term     : expr typ func
+    }.
+
+    Definition Proper_conclD (tus tvs : tenv typ) (p : Proper_concl)
+    : option (exprT tus tvs Prop) :=
+      match typeof_expr tus tvs p.(term) with
+      | Some t =>
+        match RD RbaseD p.(relation) t
+            , exprD' tus tvs t p.(term)
+        with
+        | Some rD , Some eD =>
+          Some (fun us vs => rD (eD us vs) (eD us vs))
+        | _ , _ => None
+        end
+      | None => None
+      end.
+
+    Definition Proper_lemma := Lemma.lemma typ (expr typ func) Proper_concl.
+
+    (* This splits a relation into a relation arity and a relation *)
+    Fixpoint split_R (r : R) : list R * R :=
+      match r with
+      | Rrespects l r =>
+        let (ls, r) := split_R r in
+        (l :: ls, r)
+      | _ => (nil, r)
+      end.
+
+    Lemma split_R_sound : forall r_end r rs,
+        split_R r = (rs, r_end) ->
+        fold_right Rrespects r_end rs = r.
+    Proof using.
+      induction r; simpl; intros; inv_all; subst; simpl; try reflexivity.
+      destruct (split_R r2). inv_all. subst.
+      specialize (IHr2 _ eq_refl).
+      simpl. rewrite IHr2. reflexivity.
+    Qed.
+
+    Require Import MirrorCore.RTac.CoreK.
+
+    Definition apply_respectful (lem : Proper_lemma)
+               (tacK : rtacK typ (expr typ func))
+    : expr typ func -> R -> mrw (list R) :=
+      let (rs,r_final) := split_R lem.(Lemma.concl).(relation) in
+      match lem.(Lemma.vars) with
+      | nil => match lem.(Lemma.premises) with
+               | nil => fun e r =>
+                          match expr_sdec e lem.(Lemma.concl).(term)
+                                , Req_dec Rbase_eq r r_final
+                          with
+                          | true , true => rw_ret rs
+                          | _ , _ => rw_fail
+                          end
+               | _ :: _ => fun e r =>
+                             (** TODO(gmalecha): Handle this *)
+                             rw_fail
+               end
+      | _ :: _ => fun _ _ => (** TODO(gmalecha): Handle this *)
+                    rw_fail
+      end.
+
+    Theorem apply_respectful_sound : forall lem tacK,
+        Lemma.lemmaD Proper_conclD nil nil lem ->
+        forall Htac : rtacK_sound tacK,
+          respectful_spec (apply_respectful lem tacK).
+    Proof.
+      red; intros.
+      unfold apply_respectful in H0.
+      consider (split_R (relation (Lemma.concl lem))); intros.
+      destruct (Lemma.vars lem) eqn:?.
+      { destruct (Lemma.premises lem) eqn:?; try solve [ inversion H2 ].
+        generalize (expr_sdec_sound e lem.(Lemma.concl).(term)).
+        generalize (Req_dec_ok Rbase_eq Rbase_eq_ok r r0).
+        destruct (expr_sdec e (term (Lemma.concl lem))); try solve [ inversion H2 ].
+        destruct (Req_dec Rbase_eq r r0); try solve [ inversion H2 ].
+        unfold rw_ret in H2. inv_all.
+        intros. specialize (H2 eq_refl). specialize (H5 eq_refl).
+        subst.
+        split; auto. intros.
+        forward.
+        red in H.
+        simpl in H.
+        unfold Lemma.lemmaD' in H.
+        forwardy. inv_all. subst.
+        generalize dependent lem.(Lemma.vars); intros; subst.
+        generalize dependent lem.(Lemma.premises); intros; subst.
+        simpl in *.
+        unfold Proper_conclD in H6.
+        forwardy.
+        inv_all. subst.
+        simpl in *.
+        erewrite split_R_sound by eassumption.
+        destruct (ExprFacts.exprD'_weaken _ _ _ (getUVars ctx) (tvs'++getVars ctx) H8) as [ ? [ ? ? ] ].
+        simpl in H.
+        generalize (@exprD'_deterministic _ _ _ _ _ _ _ _ _ _ _ _ _ _ _ H H4).
+        unfold Rty. intros.
+        revert H5.
+        subst y. intros.
+        rewrite H7.
+        split; [ reflexivity | ].
+        intros.
+        eapply Pure_pctxD; eauto.
+        intros.
+        specialize (@H9 HList.Hnil HList.Hnil us0 (HList.hlist_app vs' vs0)); simpl in H9.
+        rewrite H9 in H5.
+        rewrite H4 in H.
+        inv_all. subst. eapply H5. }
+      { inversion H2. }
+    Qed.
+
+    Definition apply_prespectful {T : Type}
+               (get : expr typ func -> R -> option T)
+               (lem : T -> Proper_lemma) (tacK : rtacK _ _)
+    : expr typ func -> R -> mrw (list R) :=
+      fun e r =>
+        match get e r with
+        | Some t => apply_respectful (lem t) tacK e r
+        | _ => rw_fail
+        end.
+
+    Theorem apply_prespectful_sound : forall {T} get (lem : T -> _) (tacK : _),
+        (forall x, Lemma.lemmaD Proper_conclD nil nil (lem x)) ->
+        rtacK_sound tacK ->
+        respectful_spec (apply_prespectful get lem tacK).
+    Proof.
+      intros. unfold apply_prespectful.
+      red. intros.
+      destruct (get e r); try solve [ inversion H1 ].
+      eapply apply_respectful_sound; eauto.
+    Qed.
+
+    Definition or_respectful
+               (a b : expr typ func -> R -> mrw (list R))
+    : expr typ func -> R -> mrw (list R) :=
+      fun e r => rw_orelse (a e r) (b e r).
+
+    Theorem or_respectful_sound : forall a b,
+        respectful_spec a ->
+        respectful_spec b ->
+        respectful_spec (or_respectful a b).
+    Proof.
+      unfold or_respectful. intros.
+      red. intros.
+      eapply rw_orelse_case in H1; destruct H1; [ eapply H | eapply H0 ];
+      eassumption.
+    Qed.
+
+    Definition fail_respectful : expr typ func -> R -> mrw (list R) :=
+      fun _ _ => rw_fail.
+
+    Theorem fail_respectful_sound : respectful_spec fail_respectful.
+    Proof using.
+      red. intros. inversion H.
+    Qed.
+
+    Require Import MirrorCore.RTac.IdtacK.
+
+    Fixpoint do_respectful (propers : list (expr typ func * R))
+    : expr typ func -> R -> mrw (list R) :=
+      match propers with
+      | nil => fail_respectful
+      | (f,rel) :: propers =>
+        or_respectful
+          (apply_respectful {| vars := nil
+                             ; premises := nil
+                             ; concl := {| relation := rel
+                                         ; term := f |}
+                             |} IDTACK)
+          (fun x => do_respectful propers x)
+      end.
+
+    Theorem do_respectful_sound
+    : forall propers,
+        Forall (fun er =>
+                  let '(e,r) := er in
+                  match typeof_expr nil nil e with
+                  | None => False
+                  | Some t =>
+                    match RD RbaseD r t
+                        , exprD' nil nil e t
+                    with
+                    | Some rD , Some eD =>
+                      Proper rD (eD Hnil Hnil)
+                    | _ , _ => False
+                    end
+                  end) propers ->
+        respectful_spec (do_respectful propers).
+    Proof.
+      induction 1.
+      { eapply fail_respectful_sound. }
+      { simpl. destruct x. eapply or_respectful_sound.
+        { apply apply_respectful_sound.
+          { clear - H.
+            red. simpl. unfold lemmaD'. simpl.
+            unfold Proper_conclD. simpl.
+            forward. change_rewrite H1. apply H2. }
+          { apply IDTACK_sound. } }
+        { eauto. } }
+    Qed.
+
+  End get_respectful.
+
 End setoid.
 
-(* This fast-path eliminates the need to build environments when unification is definitely going to fail
+(* This fast-path eliminates the need to build environments when
+ * unification is definitely going to fail
     Fixpoint checkUnify (e1 e2 : expr typ func) : bool :=
       match e1 , e2 with
       | ExprCore.UVar _ , _ => true
