theories/Util/HListBuild.v
@@ -1,0 +1,63 @@
+Require Import Coq.Lists.List.
+Require Import ExtLib.Data.HList.
+Require Import ExtLib.Tactics.
+
+Set Implicit Arguments.
+Set Strict Implicit.
+
+Section hlist_build_option.
+  Context {T : Type} (F : T -> Type).
+  Context {U : Type}.
+  Variable (f : forall x : T, U -> option (F x)).
+
+  Fixpoint hlist_build_option (ls : list T) (ls' : list U)
+  : option (hlist F ls) :=
+    match ls as ls , ls' return option (hlist F ls) with
+    | nil , nil => Some Hnil
+    | l :: ls , l' :: ls' =>
+      match hlist_build_option ls ls' with
+      | None => None
+      | Some res =>
+        match f l l' with
+        | None => None
+        | Some x =>
+          Some (Hcons x res)
+        end
+      end
+    | _ , _ => None
+    end.
+
+  Lemma hlist_build_option_app_if
+    : forall a b c d e f,
+      length a = length c ->
+      hlist_build_option (a ++ b) (c ++ d) = Some (hlist_app e f) ->
+      hlist_build_option a c = Some e /\
+      hlist_build_option b d = Some f.
+  Proof.
+    clear.
+    induction a; simpl; intros.
+    { intuition; destruct c; simpl in *; try congruence.
+      rewrite (hlist_eta e). reflexivity.
+      rewrite (hlist_eta e) in H0. simpl in H0. assumption. }
+    { destruct c; simpl in *; try congruence.
+      inversion H; clear H; subst.
+      forward. inv_all.
+      rewrite (hlist_eta e) in *.
+      simpl in *.
+      inv_all. subst.
+      eapply IHa in H; auto.
+      destruct H. rewrite H. eauto. }
+  Qed.
+
+  Lemma hlist_build_option_app_only_if
+  : forall a b c d e f,
+      hlist_build_option a c = Some e ->
+      hlist_build_option b d = Some f ->
+      hlist_build_option (a ++ b) (c ++ d) = Some (hlist_app e f).
+  Proof.
+    induction a; simpl; intros; forward.
+    { rewrite (hlist_eta e). simpl. auto. }
+    { inv_all; subst.
+      simpl. eapply IHa in H0; eauto. rewrite H0. rewrite H2. reflexivity. }
+  Qed.
+End hlist_build_option.
